Simplify indirect block rep and re-prove functions
Instead of keeping track of the number of valid blocks at each level of the
tree, and avoiding specifying anything about the invalid blocks, this rep
specifies the full tree, specifying that any 0 entries "point" to a virtual
all-zero block. This makes the functions much easier to prove, as eliminates
the need to change the predicate mapped by listmatch, which was painful under
the previous scheme. Since the tree is fully specified at all times, this should
make it fairly easy to support sparse files at the block level in the future.
The eventual goal is to specify and prove the following operations
on indirect blocks:
  - get  : get the block number at a specified index in the linear block list
  - read : read the entire linear block list
  - put  : set the block number at a specified index to a nonzero value
  - clear: set the block number at a specified index to 0 - this should
           also reclaim unneeded indirect blocks.

This patch specifies and proves the first three operations, though the proof for
`put` is quite messy and will be cleaned up in another commit.

src/BlockPtr.v
@@ -160,29 +160,22 @@ Module BlockPtr (BPtr : BlockPtrSig).
 
   (************** rep invariant *)
 
-   Definition indrep_n_helper bxp ibn iblocks nvalid :=
-    (if (addr_eq_dec nvalid 0)
-      then [[ length iblocks = NIndirect ]]
+   Definition indrep_n_helper bxp ibn iblocks :=
+    (if (addr_eq_dec ibn 0)
+      then [[ iblocks = repeat $0 NIndirect ]]
       else [[ BALLOC.bn_valid bxp ibn ]] * IndRec.rep ibn iblocks
     )%pred.
-
-  Definition index_nvalid indlvl' nvalid index :=
-    let divisor := NIndirect ^ S indlvl' in
-    nvalid - index * divisor.
 
   (* indlvl = 0 if ibn is the address of an indirect block,
      indlvl = 1 for doubly indirect, etc. *)
 
- Fixpoint indrep_n_tree indlvl bxp ibn l nvalid :=
+  Fixpoint indrep_n_tree indlvl bxp ibn l :=
     (match indlvl with
-    | 0 => indrep_n_helper bxp ibn l nvalid
+    | 0 => indrep_n_helper bxp ibn l
     | S indlvl' => let divisor := NIndirect ^ indlvl in
                     exists iblocks l_part, [[ l = concat l_part ]] *
-                    indrep_n_helper bxp ibn iblocks (divup nvalid divisor) *
-                    listmatch (fun index_ibn' l' => let '(index, ibn') := index_ibn' in
-                        indrep_n_tree indlvl' bxp (# ibn') l'
-                          (index_nvalid indlvl' nvalid index))
-                      (enumerate iblocks) l_part
+                    indrep_n_helper bxp ibn iblocks *
+                    listmatch (fun ibn' l' => indrep_n_tree indlvl' bxp (# ibn') l') iblocks l_part
     end)%pred.
 
   Hint Extern 0 (okToUnify (listmatch _ _ _) (listmatch _ _ _)) => constructor : okToUnify.
@@ -190,7 +183,7 @@ Module BlockPtr (BPtr : BlockPtrSig).
 
   Definition indrep bxp ir (indlist : list waddr) nblocks :=
     ( [[ nblocks = 0 ]] \/ (
-      [[ nblocks > 0 ]] * indrep_n_tree 0 bxp (IRIndPtr ir) indlist nblocks))%pred.
+      [[ nblocks > 0 ]] * indrep_n_tree 0 bxp (IRIndPtr ir) indlist))%pred.
 
   Definition rep bxp (ir : irec) (l : list waddr) :=
     ( [[ length l = (IRLen ir) /\ length l <= NBlocks ]] *
@@ -206,15 +199,15 @@ Module BlockPtr (BPtr : BlockPtrSig).
   Definition rep_indirect bxp (ir : irec) (l : list waddr) :=
     ( [[ length l = (IRLen ir) /\ length l <= NBlocks /\ length l > NDirect ]] *
       [[ length (IRBlocks ir) = NDirect ]] *
-      exists indlist, indrep_n_tree 0 bxp (IRIndPtr ir) indlist (length l - NDirect) *
+      exists indlist, indrep_n_tree 0 bxp (IRIndPtr ir) indlist *
       [[ l = (IRBlocks ir) ++ firstn (length l - NDirect) indlist ]] )%pred.
 
   (* Necessary to make subst work when there's a recursive term like:
      l = firstn (length l) ... *)
   Set Regular Subst Tactic.
 
-  Lemma indrep_n_helper_0 : forall bxp ibn l,
-    indrep_n_helper bxp ibn l 0 <=p=> [[ length l = NIndirect ]] * emp.
+  Lemma indrep_n_helper_0 : forall bxp l,
+    indrep_n_helper bxp 0 l <=p=> [[ l = repeat $0 NIndirect ]] * emp.
   Proof.
     unfold indrep_n_helper; intros; split; cancel.
   Qed.
@@ -734,85 +727,85 @@ Module BlockPtr (BPtr : BlockPtrSig).
 
   Local Hint Extern 1 (Nat.divide ?a ?b) => divide_mult.
 
-  Fact nvalid_gt_0_indrep_helper : forall bxp bn l nvalid, nvalid > 0 ->
-    indrep_n_helper bxp bn l nvalid <=p=> [[BALLOC.bn_valid bxp bn]] * IndRec.rep bn l.
-  Proof.
-    unfold indrep_n_helper; intros; destruct addr_eq_dec; simpl; solve [omega | auto].
-  Qed.
-
-  Lemma indrep_n_helper_length : forall bxp ibn l nvalid m,
-    indrep_n_helper bxp ibn l nvalid m -> length l = NIndirect.
+  Lemma indrep_n_helper_length : forall bxp ibn l m,
+    indrep_n_helper bxp ibn l m -> length l = NIndirect.
   Proof.
     unfold indrep_n_helper, IndRec.rep, IndRec.items_valid.
     intros; destruct addr_eq_dec; destruct_lift H; unfold lift_empty in *;
     intuition; subst; autorewrite with lists; auto.
+    unfold IndRec.Defs.item in *; simpl in *. omega.
   Qed.
 
-  Lemma indrep_n_helper_length_piff : forall bxp ibn l nvalid,
-    indrep_n_helper bxp ibn l nvalid <=p=> indrep_n_helper bxp ibn l nvalid * [[ length l = NIndirect ]].
+  Lemma indrep_n_helper_length_piff : forall bxp ibn l,
+    indrep_n_helper bxp ibn l <=p=> indrep_n_helper bxp ibn l * [[ length l = NIndirect ]].
   Proof.
     intros.
     split; [> intros m H; apply indrep_n_helper_length in H as HH; pred_apply | ]; cancel.
   Qed.
 
-  Lemma indrep_n_tree_listmatch_lift_helper : forall indlvl nvalid bxp index (ibn : waddr) y,
-    (fun n_w y => indrep_n_tree indlvl bxp # (snd n_w) y (nvalid - (fst n_w) * (NIndirect * NIndirect ^ indlvl)))
-      (index, ibn) y <=p=> indrep_n_tree indlvl bxp # (ibn) y (nvalid - index * (NIndirect * NIndirect ^ indlvl)).
-  Proof.
-    intros; simpl.
-    apply piff_refl.
-  Qed.
-
-  Lemma indrep_n_length_pimpl : forall indlvl bxp ibn l nvalid,
-    indrep_n_tree indlvl bxp ibn l nvalid <=p=>
-    [[ length l = NIndirect ^ (S indlvl) ]] * indrep_n_tree indlvl bxp ibn l nvalid.
+  Lemma indrep_n_length_pimpl : forall indlvl bxp ibn l,
+    indrep_n_tree indlvl bxp ibn l <=p=>
+    [[ length l = NIndirect ^ (S indlvl) ]] * indrep_n_tree indlvl bxp ibn l.
   Proof.
     induction indlvl; simpl; intros.
     intros; split; intros m H; destruct_lift H; pred_apply; cancel.
     erewrite indrep_n_helper_length; eauto; omega.
     intros; split; intros m H; destruct_lift H; pred_apply; cancel.
     rewrite indrep_n_helper_length_piff, listmatch_length_pimpl in H; destruct_lift H.
-    rewrite length_enumerate in *.
     rewrite listmatch_lift_r in H; destruct_lift H.
     erewrite concat_hom_length; eauto.
     f_equal; omega.
-    intros x y; destruct x.
-    rewrite indrep_n_tree_listmatch_lift_helper.
+    intros x y.
     split; [> rewrite IHindlvl |]; cancel.
   Qed.
 
-  Lemma indrep_index_length_helper_l : forall Fm off nvalid indlvl bxp bn iblocks l_part m f,
+  Lemma indrep_n_tree_length: forall indlvl F ir l1 l2 bxp m, (F *
+    indrep_n_helper bxp ir l1 *
+    listmatch
+     (fun ibn' l' => indrep_n_tree indlvl bxp # (ibn') l') l1 l2)%pred m->
+     length (concat l2) = NIndirect * (NIndirect ^ (S indlvl)).
+  Proof.
+    intros.
+    rewrite indrep_n_helper_length_piff in H.
+    rewrite listmatch_length_pimpl in H.
+    erewrite listmatch_lift_r in H.
+    destruct_lift H.
+    erewrite concat_hom_length; eauto.
+    f_equal; omega.
+    intros.
+    rewrite indrep_n_length_pimpl. split; cancel.
+  Qed.
+
+  Lemma indrep_index_bound_helper : forall Fm off indlvl bxp bn iblocks l_part m,
     off < length (concat l_part) ->
-    ((Fm * indrep_n_helper bxp bn iblocks nvalid) *
-          listmatch (fun (index_ibn' : addr * waddr) (l' : list waddr) =>
-           let '(index, ibn') := index_ibn' in
-            indrep_n_tree indlvl bxp # (ibn') l' (f index))
-          (enumerate iblocks) l_part)%pred m
-    -> off / (NIndirect * NIndirect ^ indlvl) < length (iblocks).
+    ((Fm * indrep_n_helper bxp bn iblocks) *
+          listmatch (fun ibn' (l' : list waddr) =>
+            indrep_n_tree indlvl bxp # (ibn') l') iblocks l_part)%pred m
+    -> off / (NIndirect * NIndirect ^ indlvl) < NIndirect.
   Proof.
     intros.
     apply Nat.div_lt_upper_bound; mult_nonzero.
-    rewrite listmatch_length_pimpl, listmatch_lift_r in *.
-    rewrite indrep_n_helper_length_piff in *.
-    rewrite length_enumerate in *.
-    destruct_lifts.
-    match goal with
-    | [ H : ?off < length (concat ?l) |- _] => erewrite concat_hom_length in H by eauto
-    end.
-    rewrite mult_comm.
-    substl (length iblocks); eauto.
-    intros x y. destruct x. intros.
-    instantiate (1 := fun x y => indrep_n_tree indlvl bxp (# (snd x)) y (f (fst x))).
-    rewrite indrep_n_length_pimpl; split; cancel.
+    erewrite indrep_n_tree_length in * by eauto.
+    rewrite mult_comm; simpl in *. auto.
   Qed.
 
-  Lemma indrep_index_length_helper_l' : forall Fm Fm' off nvalid indlvl bxp bn iblocks l_part m f,
+  Lemma indrep_index_length_helper_l : forall Fm off indlvl bxp bn iblocks l_part m,
     off < length (concat l_part) ->
-    ((Fm * indrep_n_helper bxp bn iblocks nvalid) *
-          listmatch (fun (index_ibn' : addr * waddr) (l' : list waddr) =>
-           let '(index, ibn') := index_ibn' in
-            indrep_n_tree indlvl bxp # (ibn') l' (f index))
-          (enumerate iblocks) l_part * Fm')%pred m
+    ((Fm * indrep_n_helper bxp bn iblocks) *
+          listmatch (fun ibn' (l' : list waddr) =>
+            indrep_n_tree indlvl bxp # (ibn') l') iblocks l_part)%pred m
+    -> off / (NIndirect * NIndirect ^ indlvl) < length (iblocks).
+  Proof.
+    intros.
+    rewrite indrep_n_helper_length_piff in *. destruct_lifts.
+    substl (length iblocks). eapply indrep_index_bound_helper; eauto.
+  Qed.
+
+  Lemma indrep_index_length_helper_l' : forall Fm Fm' off indlvl bxp bn iblocks l_part m,
+    off < length (concat l_part) ->
+    ((Fm * indrep_n_helper bxp bn iblocks) *
+          listmatch (fun ibn' l' => indrep_n_tree indlvl bxp # (ibn') l')
+          iblocks l_part * Fm')%pred m
     -> off / (NIndirect * NIndirect ^ indlvl) < length (iblocks).
   Proof.
     intros. eapply indrep_index_length_helper_l; eauto.
@@ -820,32 +813,25 @@ Module BlockPtr (BPtr : BlockPtrSig).
     rewrite sep_star_comm, <- sep_star_assoc. apply pimpl_refl.
   Qed.
 
-  Lemma indrep_index_length_helper_r : forall Fm off nvalid indlvl bxp bn iblocks l_part m f,
+  Lemma indrep_index_length_helper_r : forall Fm off indlvl bxp bn iblocks l_part m,
     off < length (concat l_part) ->
-    ((Fm * indrep_n_helper bxp bn iblocks nvalid) *
-          listmatch (fun (index_ibn' : addr * waddr) (l' : list waddr) =>
-           let '(index, ibn') := index_ibn' in
-            indrep_n_tree indlvl bxp # (ibn') l' (f index))
-          (enumerate iblocks) l_part)%pred m
+    ((Fm * indrep_n_helper bxp bn iblocks) *
+          listmatch (fun ibn' (l' : list waddr) =>
+            indrep_n_tree indlvl bxp # (ibn') l') iblocks l_part)%pred m
     -> off / (NIndirect * NIndirect ^ indlvl) < length l_part.
   Proof.
     intros.
     rewrite listmatch_length_pimpl in *.
-    rewrite length_enumerate in *.
-    match goal with
-    | [ H : context [ lift_empty ] |- _] => destruct_lift H
-    end.
+    destruct_lifts.
     substl (length l_part).
     eapply indrep_index_length_helper_l; eauto.
   Qed.
 
-  Lemma indrep_index_length_helper_r' : forall Fm Fm' off nvalid indlvl bxp bn iblocks l_part m f,
+  Lemma indrep_index_length_helper_r' : forall Fm Fm' off indlvl bxp bn iblocks l_part m,
     off < length (concat l_part) ->
-    ((Fm * indrep_n_helper bxp bn iblocks nvalid) *
-          listmatch (fun (index_ibn' : addr * waddr) (l' : list waddr) =>
-           let '(index, ibn') := index_ibn' in
-            indrep_n_tree indlvl bxp # (ibn') l' (f index))
-          (enumerate iblocks) l_part * Fm')%pred m
+    ((Fm * indrep_n_helper bxp bn iblocks) *
+          listmatch (fun ibn' (l' : list waddr) =>
+            indrep_n_tree indlvl bxp # (ibn') l') iblocks l_part * Fm')%pred m
     -> off / (NIndirect * NIndirect ^ indlvl) < length l_part.
   Proof.
     intros. eapply indrep_index_length_helper_r; eauto.
@@ -853,301 +839,71 @@ Module BlockPtr (BPtr : BlockPtrSig).
     rewrite sep_star_comm, <- sep_star_assoc. apply pimpl_refl.
   Qed.
 
-  Theorem indrep_n_tree_nvalid_oob : forall indlvl bxp ibn l nvalid,
-    nvalid >= (NIndirect ^ S indlvl) ->
-    indrep_n_tree indlvl bxp ibn l nvalid <=p=> indrep_n_tree indlvl bxp ibn l (NIndirect ^ S indlvl).
-  Proof.
-    intros.
-    pose proof IndRec.Defs.items_per_val_gt_0'.
-    assert (NIndirect <= NIndirect ^ (S indlvl)).
-    simpl; apply mul_ge_l; solve [mult_nonzero | auto].
-    assert (nvalid > 0) by omega.
-    generalize dependent nvalid.
-    generalize dependent l.
-    generalize dependent ibn.
-    generalize dependent bxp.
-    induction indlvl; simpl; intros.
-    split; cancel; repeat rewrite nvalid_gt_0_indrep_helper by omega; cancel.
-    split; intros m H'; destruct_lift H'; repeat rewrite nvalid_gt_0_indrep_helper in * by omega;
-    match goal with [H : _ |- _] => destruct_lift H end; pred_apply; cancel.
-    all : rewrite divup_mul in * by mult_nonzero.
-    all : assert (divup nvalid (NIndirect * NIndirect ^ indlvl) > 0) by
-            (apply divup_mul_ge; mult_nonzero; rewrite mult_comm;
-             eapply le_trans; [> apply mult_le_compat_r | apply H]; auto).
-    all : repeat rewrite nvalid_gt_0_indrep_helper in * by auto.
-    all : erewrite listmatch_piff_replace; try cancel.
-    all : intros x y; destruct x; intros.
-    all : unfold IndRec.rep, IndRec.items_valid in *; destruct_lifts.
-    all : unfold enumerate in *; apply in_combine_l, in_seq in H5.
-    all : unfold IndRec.Defs.item in *; simpl in *.
-    all : split; intros mm HH.
-    all : apply IHindlvl in HH; try apply IHindlvl; eauto.
-    all : unfold index_nvalid.
-    all : repeat match goal with
-    | [ |- ?n + ?a * ?n <= _ ] => replace n with (1 * n) at 1 by omega
-    | [ |- _ - _ > _ ] => apply Nat.lt_add_lt_sub_r; simpl
-    | [ |- _ - _ >= _ ] => apply Nat.le_add_le_sub_r; simpl
-    | [ H : ?nvalid >= ?n * ?k |- _ < ?nvalid ] => eapply lt_le_trans; [> | apply H]
-    | [ H : ?nvalid >= ?n * ?k |- _ <= ?nvalid ] => eapply le_trans; [> | apply H]
-    | [ |- ?a * ?n < ?b * ?n] => apply mult_lt_compat_r
-    | [ |- ?a * ?n <= ?b * ?n] => apply mult_le_compat_r
-    | [ |- context [?a * ?n + ?b * ?n] ] => rewrite <- Nat.mul_add_distr_r
-    | [ |- _] => solve [apply mul_ge_l; mult_nonzero | omega | mult_nonzero]
-    end.
-  Qed.
-
-  Lemma indrep_n_tree_ragged_extract : forall indlvl bxp ibn l nvalid i,
-    i = nvalid / NIndirect ^ S indlvl ->
-    indrep_n_tree indlvl bxp ibn l (index_nvalid indlvl nvalid i) <=p=>
-    indrep_n_tree indlvl bxp ibn l (nvalid mod NIndirect ^ S indlvl).
-  Proof.
-    unfold index_nvalid. intros.
-    subst i.
-    rewrite sub_round_eq_mod by mult_nonzero. auto.
-  Qed.
-
-  Lemma indrep_n_tree_full_extract : forall indlvl bxp ibn l nvalid i,
-    i < nvalid / NIndirect ^ S indlvl ->
-    indrep_n_tree indlvl bxp ibn l (index_nvalid indlvl nvalid i) <=p=>
-    indrep_n_tree indlvl bxp ibn l (NIndirect ^ S indlvl).
-  Proof.
-    intros.
-    unfold index_nvalid.
-    apply indrep_n_tree_nvalid_oob.
-    apply lt_div_mul_add_le in H; mult_nonzero.
-    omega.
-  Qed.
-
-  Lemma indrep_n_tree_empty_extract : forall indlvl bxp ibn l nvalid i,
-    nvalid <= i * NIndirect ^ S indlvl ->
-    indrep_n_tree indlvl bxp ibn l (index_nvalid indlvl nvalid i) <=p=>
-    indrep_n_tree indlvl bxp ibn l 0.
-  Proof.
-    intros.
-    unfold index_nvalid.
-    replace (_ - _) with 0 by omega. auto.
-  Qed.
-
-  Lemma indrep_n_tree_length: forall indlvl F ir l1 l2 bxp nvalid n m, (F *
-    indrep_n_helper bxp ir l1 n *
-    listmatch
-     (fun index_ibn' l' => let '(index, ibn') := index_ibn' in
-       indrep_n_tree indlvl bxp # (ibn') l' (nvalid - index * (NIndirect * NIndirect ^ indlvl)))
-     (enumerate l1) l2)%pred m-> length (concat l2) = NIndirect * (NIndirect ^ (S indlvl)).
-  Proof.
-    intros.
-    rewrite indrep_n_helper_length_piff in H.
-    rewrite listmatch_length_pimpl in H.
-    erewrite listmatch_lift_r in H.
-    destruct_lift H.
-    rewrite length_enumerate in *.
-    erewrite concat_hom_length; eauto.
-    f_equal; omega.
-    intros.
-    destruct x.
-    rewrite indrep_n_tree_listmatch_lift_helper.
-    apply indrep_n_length_pimpl.
-  Qed.
-
-  Lemma indrep_n_indlist_forall_length : forall F indlvl bxp ir l1 l2 n nvalid m,
-    ((F ✶ indrep_n_helper bxp ir l1 n)
+  Lemma indrep_n_indlist_forall_length : forall F indlvl bxp ir l1 l2 m,
+    ((F ✶ indrep_n_helper bxp ir l1)
         ✶ listmatch
-            (fun (index_ibn' : addr * waddr) (l' : list waddr) =>
-             let '(index, ibn') := index_ibn' in
-              indrep_n_tree indlvl bxp # (ibn') l' (nvalid - index * (NIndirect * NIndirect ^ indlvl)))
-            (enumerate l1) l2)%pred m ->
+            (fun ibn' l' =>indrep_n_tree indlvl bxp # (ibn') l') l1 l2)%pred m ->
     Forall (fun sublist : list waddr => length sublist = NIndirect * NIndirect ^ indlvl) l2.
   Proof.
     intros.
     rewrite indrep_n_helper_length_piff, listmatch_lift_r in H.
     destruct_lifts; eauto.
-    intros x; destruct x; intros.
-    rewrite indrep_n_tree_listmatch_lift_helper.
-    apply indrep_n_length_pimpl.
+    intros x; intros.
+    rewrite indrep_n_length_pimpl. split; cancel.
   Qed.
 
   Local Hint Resolve indrep_n_indlist_forall_length.
 
-  Theorem listmatch_indrep_n_helper_valid : forall bxp l l_part f,
-    (forall x, x < length l -> f x > 0) ->
-    listmatch (fun (index_ibn' : addr * waddr) (l' : list waddr) =>
-               let '(index, ibn') := index_ibn' in
-                indrep_n_helper bxp # (ibn') l' (f index))
-              (enumerate l) l_part <=p=>
-    listmatch (fun (index_ibn' : addr * waddr) (l' : list waddr) =>
-               let '(index, ibn') := index_ibn' in
-                indrep_n_helper bxp # (ibn') l' NIndirect)
-              (enumerate l) l_part.
-  Proof.
-    intros.
-    rewrite listmatch_piff_replace.
-    apply piff_refl.
-    intros.
-    destruct x.
-    unfold indrep_n_helper.
-    unfold enumerate in *.
-    pose proof IndRec.Defs.items_per_val_not_0.
-    assert (f n > 0). apply H.
-    match goal with [H : In (_, _) (combine (seq _ _) _) |- _] =>
-      eapply in_combine_l in H; apply in_seq in H; omega
-    end.
-    repeat destruct addr_eq_dec; auto; omega.
-  Qed.
-
-  Theorem listmatch_indrep_n_helper_invalid : forall bxp a n l l_part f,
-    (forall x, x >= a -> f x = 0) ->
-    n = length l ->
-    listmatch (fun (index_ibn' : addr * waddr) (l' : list waddr) =>
-               let '(index, ibn') := index_ibn' in
-                indrep_n_helper bxp # (ibn') l' (f index))
-              (combine (seq a n) l) l_part <=p=>
-              [[ Forall (fun x => length x = NIndirect) l_part ]] * [[ length l = length l_part]].
-  Proof.
-    intros.
-    rewrite listmatch_lift_r.
-    unfold listmatch.
-    rewrite listpred_emp_piff.
-    subst; rewrite combine_length, seq_length, Nat.min_id.
-    split. cancel; eauto.
-    cancel.
-    intros x; destruct x; intros.
-    instantiate (1 := fun _ _ => emp); auto.
-    intros x; destruct x; intros.
-    unfold indrep_n_helper.
-    rewrite H; simpl.
-    split; cancel.
-    eapply in_seq, in_combine_l. eauto.
-  Qed.
-
-  Theorem listmatch_indrep_n_helper_length_piff : forall bxp iblocks l_part f,
-    listmatch (fun (index_ibn' : addr * waddr) (l' : list waddr) =>
-            let '(index, ibn') := index_ibn' in
-             indrep_n_helper bxp # (ibn') l' (f index)) iblocks l_part <=p=>
-    listmatch (fun (index_ibn' : addr * waddr) (l' : list waddr) =>
-            let '(index, ibn') := index_ibn' in
-             indrep_n_helper bxp # (ibn') l' (f index)) iblocks l_part *
-             [[ Forall (fun x : list waddr => length x = NIndirect) l_part ]].
-  Proof.
-    intros.
-    rewrite listmatch_lift_r.
-    2 : intros x; destruct x; intros.
-    2 : rewrite indrep_n_helper_length_piff.
-    2 : instantiate (2 := fun x => length x = NIndirect).
-    2 : instantiate (1 := fun n_w y => indrep_n_helper bxp (# (snd n_w)) y (f (fst n_w))).
-    2 : simpl; split; cancel.
-    split; cancel.
-  Qed.
-
-  Theorem listmatch_indrep_n_tree_replace_nvalid : forall indlvl nvalid nvalid' bxp iblocks l_part i,
-    let N := NIndirect ^ S indlvl in
-    i = nvalid / N ->
-    i = nvalid' / N ->
-    listmatch  (fun (index_ibn' : addr * waddr) l' =>
-                let '(index, ibn') := index_ibn' in
-                  indrep_n_tree indlvl bxp # (ibn') l' (index_nvalid indlvl nvalid index))
-        (removeN (enumerate iblocks) i) (removeN l_part i) <=p=>
-    listmatch  (fun (index_ibn' : addr * waddr) l' =>
-                let '(index, ibn') := index_ibn' in
-                  indrep_n_tree indlvl bxp # (ibn') l' (index_nvalid indlvl nvalid' index))
-        (removeN (enumerate iblocks) i) (removeN l_part i).
-  Proof.
-    intros. apply listmatch_piff_replace.
-    intros x; destruct x as [a b]; intros.
-    apply in_removeN_enumerate in H1.
-    unfold index_nvalid.
-    intuition.
-    repeat rewrite indrep_n_tree_nvalid_oob with (nvalid := _ - _); auto;
-    match goal with [H : i = ?nvalid / N |- ?nvalid - _ >= _] =>
-      rewrite Nat.div_mod with (x := nvalid) (y := N) by (subst N; mult_nonzero);
-      rewrite mult_comm, plus_comm; subst N;
-      rewrite <- H; rewrite <- Nat.add_sub_assoc by (apply mult_le_compat_r; omega);
-      rewrite <- Nat.mul_sub_distr_r, plus_comm;
-      apply le_plus_trans, mul_ge_r; omega
-    end.
-    repeat rewrite sub_le_eq_0; auto;
-      apply Nat.lt_le_incl; apply div_lt_mul_lt; mult_nonzero; subst N; omega.
-  Qed.
-
-  Theorem listmatch_indrep_n_tree_aligned : forall indlvl bxp n n1 l1 l2,
-    n <= length l1 ->
-    n = n1 - 1 ->
-    listmatch (fun (index_ibn' : addr * waddr) (l' : list waddr) =>
-      let '(index, ibn') := index_ibn' in 
-        indrep_n_tree indlvl bxp # (ibn') l'
-          (index_nvalid indlvl (n1 * (NIndirect ^ S indlvl)) index))
-      (removeN (enumerate l1) n) (removeN l2 n) <=p=>
-    listmatch (fun (index_ibn' : addr * waddr) (l' : list waddr) =>
-      let '(index, ibn') := index_ibn' in
-        indrep_n_tree indlvl bxp # (ibn') l'
-          (index_nvalid indlvl (n * (NIndirect ^ S indlvl)) index))
-      (removeN (enumerate l1) n) (removeN l2 n).
-  Proof.
-    intros.
-    apply listmatch_piff_replace.
-    intros. in_enumerate.
-    intuition.
-    repeat rewrite indrep_n_tree_full_extract by
-      (rewrite Nat.div_mul by mult_nonzero; omega). auto.
-    repeat rewrite indrep_n_tree_empty_extract by
-      (apply mult_le_compat_r; mult_nonzero; omega).
-    eauto.
-  Qed.
-
-  Theorem indrep_n_helper_pts_piff : forall bxp ir l nvalid,
-    nvalid > 0 ->
-    indrep_n_helper bxp ir l nvalid <=p=> [[ BALLOC.bn_valid bxp ir ]] * [[ IndRec.items_valid ir l]] *
-    (ir |-> (IndRec.Defs.block2val l, [])).
-  Proof.
-    intros.
-    rewrite nvalid_gt_0_indrep_helper by omega.
-    unfold IndRec.Defs.item, IndRec.rep, IndSig.RAStart in *; split; cancel.
-    all : unfold IndRec.items_valid, IndRec.Defs.item in *; intuition; simpl in *.
-    all : rewrite IndRec.Defs.ipack_one by (simpl; omega); cancel.
-  Qed.
-
-  Theorem indrep_n_tree_0 : forall indlvl bxp ir l,
-    indrep_n_tree indlvl bxp ir l 0 <=p=> [[length l = NIndirect ^ S indlvl]].
+  Theorem indrep_n_tree_0 : forall indlvl bxp l,
+    indrep_n_tree indlvl bxp 0 l <=p=> [[ l = repeat $0 (NIndirect ^ S indlvl)]].
   Proof.
     induction indlvl; simpl; intros.
     rewrite mult_1_r, indrep_n_helper_0; split; cancel.
-    rewrite divup_0. split.
+    split.
     intros m' H'.
     destruct_lift H'.
     rewrite indrep_n_helper_0 in H.
     rewrite listmatch_length_pimpl in H; autorewrite with lists in *.
     rewrite listmatch_lift_r with (F := fun x y => emp) in H.
-    rewrite listmatch_emp in H by auto.
+    rewrite listmatch_emp in H by cancel.
     pred_apply; cancel.
-    erewrite concat_hom_length; eauto.
-    f_equal. omega.
+    erewrite concat_hom_repeat; eauto.
+    repeat f_equal. rewrite repeat_length in *. omega.
     intros; simpl.
-    destruct x.
+    destruct_lifts. erewrite repeat_spec with (y := x); eauto.
     rewrite IHindlvl. split; cancel.
     cancel.
     instantiate (iblocks := repeat $0 NIndirect).
-    rewrite indrep_n_helper_0. rewrite repeat_length.
+    rewrite indrep_n_helper_0.
     rewrite listmatch_lift_r with (F := fun x y => emp) (P := fun y => length y = NIndirect ^ S indlvl).
     rewrite listmatch_emp_piff by auto.
     autorewrite with lists.
     cancel.
-    apply part_forall_length; try substl (length l); solve [mult_nonzero | divide_mult].
-    rewrite part_length; try substl (length l); try rewrite Nat.div_mul;
-      solve [auto | mult_nonzero | divide_mult].
-    intro x; destruct x; intros.
-    rewrite IHindlvl. split; cancel.
-    rewrite concat_hom_part; auto; mult_nonzero.
-    unfold Nat.divide. eauto.
+    apply Forall_repeat.
+    rewrite repeat_length. eauto.
+    rewrite repeat_length. eauto.
+    intro x; intros.
+    erewrite repeat_spec with (y := x); eauto.
+    rewrite IHindlvl. split; cancel. subst. autorewrite with lists. auto.
+    erewrite repeat_spec with(y := y); eauto.
+    erewrite concat_hom_repeat; autorewrite with lists.
+    rewrite plus_0_r. eauto.
+    apply Forall_repeat. auto.
   Qed.
 
   (************* n-indirect program *)
 
   Fixpoint indget (indlvl : nat) lxp (bn : addr) off ms :=
-    let divisor := NIndirect ^ indlvl in
-    let^ (ms, v) <- IndRec.get lxp bn (off / divisor) ms;
-    match indlvl with
-    | 0 => Ret ^(ms, v)
-    | S indlvl' => indget indlvl' lxp (# v) (off mod divisor) ms
-    end.
+    If (addr_eq_dec bn 0) {
+      Ret ^(ms, $ 0)
+    } else {
+      let divisor := NIndirect ^ indlvl in
+      let^ (ms, v) <- IndRec.get lxp bn (off / divisor) ms;
+      match indlvl with
+      | 0 => Ret ^(ms, v)
+      | S indlvl' => indget indlvl' lxp (# v) (off mod divisor) ms
+      end
+    }.
 
   Lemma divup_gt_0 : forall a b, 0 < a -> 0 < b -> divup a b > 0.
   Proof.
@@ -1161,7 +917,8 @@ Module BlockPtr (BPtr : BlockPtrSig).
         eapply indrep_index_length_helper_l; eauto  |
         eapply indrep_index_length_helper_l'; eauto |
         eapply indrep_index_length_helper_r; eauto  |
-        eapply indrep_index_length_helper_r'; eauto ].
+        eapply indrep_index_length_helper_r'; eauto |
+        eapply indrep_index_bound_helper; eauto].
 
   Ltac indrep_n_extract := match goal with
     | [|- context [listmatch _ ?l] ] =>
@@ -1169,16 +926,24 @@ Module BlockPtr (BPtr : BlockPtrSig).
         rewrite listmatch_isolate with (i := n) (a := l);
         autorewrite with lists in *; try omega; try erewrite snd_pair by eauto
       end
-    | [|- context [selN ?l ?n] ] => rewrite listmatch_isolate with (i := n) (a := enumerate l);
+    | [|- context [selN ?l ?n] ] => rewrite listmatch_isolate with (i := n) (a := l);
         autorewrite with lists in *; try omega; try erewrite snd_pair by eauto
   end.
 
+  (* TODO move this *)
+  Theorem indrep_n_helper_valid : forall bxp bn l,
+    bn <> 0 -> indrep_n_helper bxp bn l <=p=> [[ BALLOC.bn_valid bxp bn ]] * IndRec.rep bn l.
+  Proof.
+    intros. unfold indrep_n_helper. destruct bn; try omega. simpl.
+    split; cancel.
+  Qed.
+
   Theorem indget_ok : forall indlvl lxp bxp bn off ms,
-    {< F Fm m0 m l nvalid,
+    {< F Fm m0 m l,
     PRE:hm
            LOG.rep lxp F (LOG.ActiveTxn m0 m) ms hm *
-           [[[ m ::: Fm * indrep_n_tree indlvl bxp bn l nvalid ]]] *
-           [[ off < nvalid ]] * [[ off < length l ]]
+           [[[ m ::: Fm * indrep_n_tree indlvl bxp bn l ]]] *
+           [[ off < length l ]]
     POST:hm' RET:^(ms, r)
            LOG.rep lxp F (LOG.ActiveTxn m0 m) ms hm' *
            [[ r = selN l off $0 ]]
@@ -1188,26 +953,34 @@ Module BlockPtr (BPtr : BlockPtrSig).
   Proof.
     induction indlvl; simpl.
     + repeat safestep; autorewrite with core; eauto.
-      rewrite nvalid_gt_0_indrep_helper by omega. cancel.
+      rewrite indrep_n_helper_0 in *. destruct_lifts.
+      rewrite repeat_selN; auto. rewrite repeat_length in *. auto.
+      rewrite indrep_n_helper_valid by omega. cancel.
     + repeat safestep; autorewrite with core; try eassumption.
+      - erewrite indrep_n_tree_length in * by eauto.
+        rewrite indrep_n_helper_0, listmatch_length_pimpl in *. destruct_lifts.
+        erewrite concat_hom_repeat. rewrite repeat_selN. eauto.
+        rewrite repeat_length in *.
+        match goal with [H : _ |- _] => rewrite <- H end. eassumption.
+        rewrite listmatch_lift_r in H; destruct_lifts; eauto.
+        intros. match goal with [H : _ |- _] => apply repeat_spec in H end.
+        subst. rewrite indrep_n_tree_0. instantiate (1 := fun _ _ => emp).
+        split; cancel.
       - indrep_n_tree_bound.
-      - rewrite nvalid_gt_0_indrep_helper by (apply divup_gt_0; (omega || mult_nonzero)).
+      - rewrite indrep_n_helper_valid by omega.
         cancel.
-      - rewrite listmatch_isolate; autorewrite with lists.
-        (* these are hidden by notation, but otherwise prevent cancel from succeeding *)
-        unfold IndRec.Defs.item; simpl; erewrite snd_pair by eauto.
-        cancel.
+      - indrep_n_extract.
+        rewrite sep_star_comm. repeat rewrite <- sep_star_assoc.
+        rewrite sep_star_comm. repeat rewrite <- sep_star_assoc.
+        apply pimpl_refl.
         all : indrep_n_tree_bound.
-      - unfold index_nvalid. rewrite <- Nat.lt_add_lt_sub_r by auto.
-        rewrite plus_comm, mult_comm.
-        rewrite <- Nat.div_mod; auto.
       - match goal with [H : context [indrep_n_helper] |-_] => assert (HH := H) end.
         eapply lt_le_trans. apply Nat.mod_bound_pos; mult_nonzero; omega.
         apply Nat.eq_le_incl.
         rewrite listmatch_extract in HH; autorewrite with lists in *.
         rewrite indrep_n_length_pimpl in HH.
         destruct_lift HH. eauto.
-        all : solve [indrep_n_tree_bound].
+        solve [indrep_n_tree_bound].
       - apply selN_selN_hom.
         eapply indrep_n_indlist_forall_length; eauto.
         rewrite listmatch_length_pimpl, indrep_n_helper_length_piff in *; autorewrite with lists in *.
@@ -1215,783 +988,398 @@ Module BlockPtr (BPtr : BlockPtrSig).
         rewrite mult_comm.
         apply div_lt_mul_lt; solve [indrep_n_tree_bound | mult_nonzero].
       Unshelve.
-      all : try split; eauto.
       exact $0.
   Qed.
 
-  Fixpoint indread (indlvl : nat) lxp (ir : addr) nvalid ms :=
-    let^ (ms, indbns) <- IndRec.read lxp ir 1 ms;
-    match indlvl with
-      | 0 => Ret ^(ms, indbns)
-      | S indlvl' =>
-        let N := (NIndirect ^ (S indlvl')) in
-        r <- ForN i < divup nvalid N
-          Hashmap hm
-          Ghost [ F Fm iblocks l_part l bxp crash m0 m ]
-          Loopvar [ ms r ]
-          Invariant
-            LOG.rep lxp F (LOG.ActiveTxn m0 m) ms hm *
-            [[[ m ::: Fm * indrep_n_helper bxp ir iblocks (divup nvalid N) *
-                      listmatch (fun index_ibn' l' =>
-                        let '(index, ibn') := index_ibn' in
-                          indrep_n_tree indlvl' bxp (# ibn') l' (nvalid - index * N))
-                        (enumerate iblocks) l_part ]]] *
-            [[ r = firstn (min (i * (NIndirect ^ indlvl)) (roundup nvalid NIndirect)) l ]]
-          OnCrash crash
-          Begin
-            let nvalid' := (min (NIndirect ^ indlvl) (nvalid - i * NIndirect ^ indlvl)) in
-            let^ (ms, v) <- indread indlvl' lxp #(selN indbns i IndRec.Defs.item0) nvalid' ms;
-            Ret ^(ms, r ++ v)
-          Rof ^(ms, nil);
-          Ret r
+  Fixpoint indread (indlvl : nat) lxp (ir : addr) ms :=
+    If (addr_eq_dec ir 0) {
+      Ret ^(ms, repeat $0 (NIndirect ^ S indlvl))
+    } else {
+      let^ (ms, indbns) <- IndRec.read lxp ir 1 ms;
+      match indlvl with
+        | 0 => Ret ^(ms, indbns)
+        | S indlvl' =>
+          let N := (NIndirect ^ (S indlvl')) in
+          r <- ForN i < NIndirect
+            Hashmap hm
+            Ghost [ F Fm iblocks l_part l bxp crash m0 m ]
+            Loopvar [ ms r ]
+            Invariant
+              LOG.rep lxp F (LOG.ActiveTxn m0 m) ms hm *
+              [[[ m ::: Fm * indrep_n_helper bxp ir iblocks *
+                        listmatch (fun ibn' l' => indrep_n_tree indlvl' bxp (# ibn') l')
+                          iblocks l_part ]]] *
+              [[ r = firstn (i * (NIndirect ^ indlvl)) l ]]
+            OnCrash crash
+            Begin
+              let^ (ms, v) <- indread indlvl' lxp #(selN indbns i IndRec.Defs.item0) ms;
+              Ret ^(ms, r ++ v)
+            Rof ^(ms, nil);
+            Ret r
+      end
+    }.
+
+  (* TODO move this *)
+  Ltac cancel_last := repeat match goal with
+    | [|- _ * ?a =p=> _ * ?a] => (apply pimpl_sep_star; apply pimpl_refl || fail)
+    | [|- (_ * _) * _ =p=> _ ] => rewrite sep_star_comm
+    | [|- _ * (_ * _) =p=> _ ] => repeat rewrite <- sep_star_assoc
     end.
 
-  Theorem indread_ok : forall indlvl lxp bxp ir nvalid ms,
+  (* TODO move this and use it in indget *)
+  Theorem indrep_n_tree_repeat:
+    forall (indlvl : addr) (F : pred) (l1 : list waddr) (l2 : list (list waddr)) 
+      (bxp : balloc_xparams) (m : Mem.mem),
+    ((F ✶ indrep_n_helper bxp 0 l1)
+     ✶ listmatch (fun (ibn' : waddr) (l' : list waddr) => indrep_n_tree indlvl bxp # (ibn') l') l1 l2)%pred m ->
+    concat l2 = repeat $0 (NIndirect * NIndirect ^ S indlvl).
+  Proof.
+    intros. rewrite indrep_n_helper_0 in *. destruct_lifts.
+    rewrite listmatch_length_pimpl in *; autorewrite with lists in *; destruct_lifts.
+    erewrite concat_hom_repeat. repeat f_equal; auto.
+    rewrite listmatch_lift_r in *. destruct_lifts; eauto.
+    intros. instantiate (1 := fun _ _ => emp). erewrite repeat_spec with (y := x); eauto.
+    rewrite indrep_n_tree_0. split; cancel.
+  Qed.
+
+  Theorem indread_ok : forall indlvl lxp bxp ir ms,
   {< F Fm m0 m l,
     PRE:hm
            LOG.rep lxp F (LOG.ActiveTxn m0 m) ms hm *
-           [[[ m ::: Fm * indrep_n_tree indlvl bxp ir l nvalid ]]] *
-           [[ nvalid <= length l ]] * [[ 0 < nvalid ]]
+           [[[ m ::: Fm * indrep_n_tree indlvl bxp ir l ]]]
     POST:hm' RET:^(ms, r)
            LOG.rep lxp F (LOG.ActiveTxn m0 m) ms hm' *
-           [[ r = firstn (roundup nvalid NIndirect) l ]]
+           [[ r = l ]]
     CRASH:hm'  exists ms',
            LOG.rep lxp F (LOG.ActiveTxn m0 m) ms' hm'
-    >} indread indlvl lxp ir nvalid ms.
+    >} indread indlvl lxp ir ms.
   Proof.
     induction indlvl; simpl.
     + hoare.
-      - rewrite nvalid_gt_0_indrep_helper by auto; cancel.
+      - rewrite indrep_n_helper_0 in *. destruct_lifts. rewrite mult_1_r. auto.
+      - rewrite indrep_n_helper_valid by auto; cancel.
       - rewrite indrep_n_helper_length_piff in *.
-        destruct_lifts.
-        repeat rewrite firstn_oob; auto; try omega.
-        substl NIndirect.
-        apply roundup_ge_divisor; auto.
+        destruct_lifts. unfold IndRec.Defs.item in *; simpl in *.
+        rewrite firstn_oob by omega. auto.
     + hoare.
-      - rewrite nvalid_gt_0_indrep_helper by (apply divup_gt_0; (omega || mult_nonzero)). cancel.
-      - rewrite listmatch_length_pimpl in *; autorewrite with lists in *.
-        rewrite indrep_n_helper_length_piff in *.
-        destruct_lifts.
-        rewrite firstn_oob by omega.
-        assert (nvalid <= NIndirect ^ (S (S indlvl))) by (eapply le_trans; eauto;
-          eapply Nat.eq_le_incl, indrep_n_tree_length; eauto); simpl in *.
-        indrep_n_extract; try (eapply divup_bound_helper; eauto; omega).
-        edestruct Min.min_spec as [ [HH Hmin]|[HH Hmin] ]; rewrite Hmin; cancel.
-        rewrite indrep_n_tree_nvalid_oob; simpl; solve [cancel | omega].
-      - match goal with [H : context [indrep_n_helper] |- _] =>
-          eapply indrep_n_indlist_forall_length in H; eapply Forall_selN in H; try rewrite H
-        end.
-        apply Nat.le_min_l.
-        rewrite indrep_n_helper_length_piff, listmatch_length_pimpl in *; destruct_lifts.
-        autorewrite with lists in *.
-        eapply divup_bound_helper; [> eauto | |].
-        eapply le_trans; eauto. eapply Nat.eq_le_incl, indrep_n_tree_length. eauto.
-        unfold IndRec.Defs.item in *; simpl in *; congruence.
-      - edestruct Min.min_spec as [ [HH Hmin]|[HH Hmin] ]; rewrite Hmin; [> mult_nonzero |].
-        rewrite <- Nat.lt_add_lt_sub_r; simpl.
-        apply divup_gt; auto; mult_nonzero.
-      - rewrite min_roundup, roundup_mult.
-        rewrite indrep_n_helper_length_piff, listmatch_length_pimpl in *;
-          destruct_lifts; autorewrite with lists in *.
-        edestruct Min.min_spec as [ [HH Hmin]|[HH Hmin] ]; rewrite Hmin in *; clear Hmin.
-        --  assert (nvalid <= NIndirect ^ (S (S indlvl))) by (eapply le_trans; eauto;
-              eapply Nat.eq_le_incl, indrep_n_tree_length; eauto); simpl in *.
-            match goal with [H : ?m < divup _ _ |- _ ] =>
-              assert (m < NIndirect) by (eapply divup_bound_helper; eauto)
-            end.
-            rewrite listmatch_length_pimpl, indrep_n_helper_length_piff in *; autorewrite with lists in *.
-            destruct_lifts.
-            erewrite le_plus_minus with (m := roundup nvalid NIndirect); [> | apply Nat.lt_le_incl; eauto].
-            rewrite plus_comm, Min.plus_min_distr_l, firstn_sum_split.
-            f_equal.
-            rewrite roundup_subt_divide at 1 by solve [divide_mult | omega].
-            edestruct Min.min_spec as [ [HH' Hmin]|[HH' Hmin] ]; rewrite Hmin in *; clear Hmin.
-            ++  erewrite concat_hom_subselect_firstn by (eauto; omega).
-                rewrite concat_hom_skipn; eauto.
-            ++  rewrite concat_hom_skipn; eauto.
-                erewrite concat_hom_subselect_firstn; eauto; omega.
-        --  pose proof roundup_ge nvalid NIndirect IndRec.Defs.items_per_val_gt_0.
-            replace (nvalid - _ * _) with 0 by omega.
-            rewrite roundup_0, min_r, app_nil_r by (apply Peano.le_0_n).
-            rewrite min_r by lia. auto.
-      - rewrite min_r; auto.
-        apply roundup_mult_mono; solve [mult_nonzero | divide_mult].
+      - erewrite indrep_n_tree_repeat; eauto. auto.
+      - rewrite indrep_n_helper_valid by omega. cancel.
+      - rewrite indrep_n_helper_length_piff. cancel.
+        rewrite firstn_oob by (unfold IndRec.Defs.item in *; simpl in *; omega).
+        indrep_n_extract.
+        cancel_last.
+        rewrite listmatch_length_pimpl in *. destruct_lifts. omega.
+      - rewrite indrep_n_helper_length_piff, listmatch_length_pimpl in *; destruct_lifts.
+        rewrite concat_hom_firstn by eauto.
+        match goal with [|- context [selN ?l ?n ?d] ] =>
+          replace (selN l n d) with (concat [selN l n d]) by (simpl; rewrite app_nil_r; auto)
+        end. rewrite <- concat_app.
+        rewrite <- firstn_plusone_selN by omega.
+        erewrite <- concat_hom_firstn by eauto. rewrite plus_comm. simpl. auto.
+      - apply firstn_oob.
+        erewrite indrep_n_tree_length by eauto. auto.
       - apply LOG.rep_hashmap_subset; eauto.
-    Unshelve. all : eauto; split; solve [eauto | exact ($0)].
+    Grab Existential Variables. all : eauto; split; solve [eauto | exact ($0)].
   Qed.
+Check (updN (repeat $0 NIndirect) 3 $ 5).
 
-  Fixpoint indshrink_clear indlvl lxp bxp ir ms :=
-    match indlvl with
-    | 0 => ms <- BALLOC.free lxp bxp ir ms;
-           Ret ^(ms)
-    | S indlvl' =>
-        let N := (NIndirect ^ S indlvl') in
-        let^ (ms, indbns) <- IndRec.read lxp ir 1 ms;
-        let^ (ms) <- ForN i < NIndirect
-          Hashmap hm
-          Ghost [ F Fm bxp crash m0 freelist l_part]
-          Loopvar [ ms ]
-          Invariant
-            exists freelist' m, LOG.rep lxp F (LOG.ActiveTxn m0 m) ms hm *
-            [[[ m ::: Fm *
-                      listmatch (fun index_ibn' l' => let '(index, ibn') := index_ibn' in
-                          indrep_n_tree indlvl' bxp (# ibn') l' (index_nvalid indlvl' ((NIndirect - i) * N) index))
-                        (enumerate indbns) l_part *
-              BALLOC.rep bxp freelist' ]]] * [[ incl freelist freelist' ]]
-          OnCrash crash
-          Begin
-            let bn := # (selN indbns (NIndirect - 1 - i) $0) in
-            let^ (ms) <- indshrink_clear indlvl' lxp bxp bn ms;
-            Ret ^(ms)
-          Rof ^(ms);
-          ms <- BALLOC.free lxp bxp ir ms;
-          Ret ^(ms)
-      end.
+  Definition indput_upd_if_necessary lxp ir v indbns to_grow ms := 
+    If (addr_eq_dec v #(selN indbns to_grow $0)) {
+      Ret ms
+    } else {
+      IndRec.write lxp ir (indbns ⟦ to_grow := ($ v)⟧) ms
+    }.
 
-  Theorem indshrink_clear_ok : forall indlvl lxp bxp ir l ms,
-    {< F Fm m0 m freelist,
+  Theorem indput_upd_if_necessary_ok : forall lxp ir v indbns to_grow ms,
+    {< F Fm m0 m bxp,
     PRE:hm
-           LOG.rep lxp F (LOG.ActiveTxn m0 m) ms hm *
-           [[[ m ::: (Fm * indrep_n_tree indlvl bxp ir l (NIndirect ^ S indlvl) * BALLOC.rep bxp freelist) ]]]
-    POST:hm' RET:^(ms)  exists m' freelist',
-           LOG.rep lxp F (LOG.ActiveTxn m0 m') ms hm' *
-           [[[ m' ::: (Fm * indrep_n_tree indlvl bxp ir l 0 * BALLOC.rep bxp freelist') ]]] *
-           [[ incl freelist freelist' ]]
+           LOG.rep lxp F (LOG.ActiveTxn m0 m) ms hm * [[ BALLOC.bn_valid bxp ir ]] *
+           [[[ m ::: (Fm * indrep_n_helper bxp ir indbns) ]]]
+    POST:hm' RET: ms
+           exists m' indbns', LOG.rep lxp F (LOG.ActiveTxn m0 m') ms hm' *
+           [[ indbns' = updN indbns to_grow ($ v) ]] *
+           [[[ m' ::: (Fm * indrep_n_helper bxp ir indbns') ]]]
     CRASH:hm'  LOG.intact lxp F m0 hm'
-    >} indshrink_clear indlvl lxp bxp ir ms.
+    >} indput_upd_if_necessary lxp ir v indbns to_grow ms.
   Proof.
-    induction indlvl.
-    + simpl. repeat rewrite mult_1_r. hoare.
-      - rewrite nvalid_gt_0_indrep_helper in * by auto.
-        destruct_lifts. auto.
-      - rewrite indrep_n_helper_0, indrep_n_helper_length_piff, indrep_n_helper_pts_piff by auto.
-        cancel.
-    + simpl.
-      rewrite divup_mul by mult_nonzero.
-      safestep.
-      rewrite nvalid_gt_0_indrep_helper by auto. cancel.
-      (* instantiate the list of indirect blocks before stepping so that it is in scope *)
-      rewrite indrep_n_helper_length_piff, listmatch_length_pimpl in *;
-        autorewrite with lists in *. destruct_lifts.
-      rewrite firstn_oob by omega.
-      repeat safestep.
-      - rewrite Nat.sub_0_r. solve [repeat cancel].
-      - apply incl_refl.
-      - eauto.
-      - indrep_n_extract. rewrite indrep_n_tree_full_extract. cancel.
-        rewrite Nat.div_mul by mult_nonzero. omega.
-      - indrep_n_extract. rewrite indrep_n_tree_empty_extract. cancel.
-        rewrite <- Nat.sub_add_distr; simpl in *.
-        apply listmatch_indrep_n_tree_aligned; try omega.
-        unfold IndRec.Defs.item in *; simpl in *. omega.
-        apply Nat.eq_le_incl. f_equal; omega.
-      - eapply incl_tran; eauto.
-      - cancel.
-      - rewrite nvalid_gt_0_indrep_helper in * by auto. destruct_lifts. auto.
-      - rewrite Nat.sub_diag. unfold index_nvalid. simpl.
-        rewrite divup_0, indrep_n_helper_0. cancel.
-        rewrite indrep_n_helper_pts_piff by auto. cancel.
-      - auto.
-      - apply incl_tl; eapply incl_tran, incl_refl; eauto.
-      - eauto.
-      - cancel.
-      - cancel. apply LOG.intact_hashmap_subset; auto.
-      - cancel. apply LOG.active_intact.
-      Grab Existential Variables.
-      all : eauto; try split; eauto.
+    unfold indput_upd_if_necessary. unfold BALLOC.bn_valid.
+    hoare.
+    rewrite natToWord_wordToNat. rewrite updN_selN_eq. cancel.
+    unfold IndRec.items_valid, IndSig.xparams_ok, IndSig.RAStart, IndSig.RALen.
+    unfold Rec.well_formed. simpl. intuition.
+    rewrite length_updN. rewrite indrep_n_helper_length_piff in *. destruct_lifts.
+    omega.
+    rewrite indrep_n_helper_valid by omega. cancel.
+    rewrite indrep_n_helper_valid by omega. cancel.
+    unfold BALLOC.bn_valid. intuition.
   Qed.
 
-  Hint Extern 1 ({{_}} Bind (indshrink_clear _ _ _ _ _) _) => apply indshrink_clear_ok : prog.
+  Local Hint Extern 0 ({{_}} Bind (indput_upd_if_necessary _ _ _ _ _ _) _) => apply indput_upd_if_necessary_ok : prog.
 
-  Definition indshrink_aligned indlvl lxp bxp (iblocks : list waddr) nvalid nr ms :=
-    let nvalid_children := nvalid / (NIndirect ^ indlvl) in
-    let nr_children := nr / (NIndirect ^ indlvl) in
-    let N := (NIndirect ^ indlvl) in
-    let^ (ms) <- ForN i < nr_children
-    Hashmap hm
-    Ghost [ F Fm bxp crash m0 freelist l_part iblocks ]
-    Loopvar [ ms ]
-    Invariant
-      exists freelist' m, LOG.rep lxp F (LOG.ActiveTxn m0 m) ms hm *
-      let bn := selN iblocks (nvalid_children - 1 - i) IndRec.Defs.item0 in
-      [[[ m ::: Fm *
-                listmatch (fun index_ibn' l' => let '(index, ibn') := index_ibn' in
-                    indrep_n_tree (indlvl - 1) bxp (# ibn') l' (index_nvalid (indlvl - 1) ((nvalid_children - i) * N) index))
-                  (enumerate iblocks) l_part *
-        BALLOC.rep bxp freelist' ]]] * [[ incl freelist freelist' ]]
-    OnCrash crash
-    Begin
-      let bn := selN iblocks (nvalid_children - 1 - i) $0 in
-      let^ (ms) <- indshrink_clear (indlvl - 1) lxp bxp #bn ms;
-      Ret ^(ms)
-    Rof ^(ms);
-    Ret ^(ms).
+  Definition indput_get_blocks {P} {Q} lxp (is_alloc : {P} + {Q}) ir ms :=
+    If (is_alloc) {
+      Ret ^(ms, repeat $0 NIndirect)
+    } else {
+      IndRec.read lxp ir 1 ms
+    }.
 
-
-  Theorem indshrink_aligned_ok : forall indlvl lxp bxp iblocks l_part nvalid nr ms,
-    let N := NIndirect ^ indlvl in
-    {< F Fm m0 m freelist,
+  Theorem indput_get_blocks_ok : forall P Q lxp (is_alloc : {P} + {Q}) ir ms,
+    {< F Fm m0 m bxp indbns,
     PRE:hm
-           LOG.rep lxp F (LOG.ActiveTxn m0 m) ms hm *
-           [[ indlvl > 0 ]] * [[ Nat.divide N nvalid ]] * [[ Nat.divide N nr ]] *
-           [[[ m ::: (Fm *
-                listmatch (fun index_ibn' l' => let '(index, ibn') := index_ibn' in
-                    indrep_n_tree (indlvl - 1) bxp (# ibn') l' (index_nvalid (indlvl - 1) nvalid index))
-                  (enumerate iblocks) l_part * BALLOC.rep bxp freelist) ]]] *
-           [[ length iblocks = NIndirect ]] * [[ nr <= nvalid <= NIndirect * N ]]
-    POST:hm' RET:^(ms)  exists m' freelist' nvalid',
-           [[ nvalid' = nvalid - nr ]] *
-           LOG.rep lxp F (LOG.ActiveTxn m0 m') ms hm' *
-           [[[ m' ::: (Fm *
-                listmatch (fun index_ibn' l' => let '(index, ibn') := index_ibn' in
-                    indrep_n_tree (indlvl - 1) bxp (# ibn') l' (index_nvalid (indlvl - 1) nvalid' index))
-                  (enumerate iblocks) l_part * BALLOC.rep bxp freelist') ]]] *
-           [[ incl freelist freelist' ]]
+           LOG.rep lxp F (LOG.ActiveTxn m0 m) ms hm * [[ BALLOC.bn_valid bxp ir ]] *
+           [[ P -> ir = 0 ]] * [[ Q -> ir <> 0 ]] *
+           [[[ m ::: (Fm * indrep_n_helper bxp ir indbns) ]]]
+    POST:hm' RET:^(ms, r)
+           LOG.rep lxp F (LOG.ActiveTxn m0 m) ms hm' * [[ r = indbns ]]
     CRASH:hm'  LOG.intact lxp F m0 hm'
-    >} indshrink_aligned indlvl lxp bxp iblocks nvalid nr ms.
+    >} indput_get_blocks lxp is_alloc ir ms.
     Proof.
-      unfold indshrink_aligned.
-      unfold Nat.divide.
-      repeat safestep;
-        repeat rewrite Nat.div_mul in * by mult_nonzero;
-        repeat rewrite <- Nat.mul_le_mono_pos_r in * by mult_nonzero.
-      - rewrite Nat.sub_0_r. cancel.
-      - apply incl_refl.
-      - eauto.
-      - rewrite listmatch_length_pimpl; cancel.
-        indrep_n_extract.
-        rewrite indrep_n_tree_full_extract. cancel.
-        replace (S (indlvl - 1)) with indlvl by omega.
-        rewrite Nat.div_mul by mult_nonzero. omega.
-      - match goal with [H : context [listmatch _ (enumerate _)] |- _] =>
-          rewrite listmatch_length_pimpl in H; destruct_lift H
-        end.
-        indrep_n_extract.
-        rewrite indrep_n_tree_empty_extract.
-        rewrite <- Nat.sub_add_distr. cancel.
-        replace indlvl with (S (indlvl - 1)) by omega. simpl. rewrite Nat.sub_0_r.
-        apply listmatch_indrep_n_tree_aligned; omega.
-        replace (S (indlvl - 1)) with indlvl by omega.
-        apply Nat.eq_le_incl. f_equal. omega.
-      - eapply incl_tran; eauto.
-      - cancel.
-      - rewrite Nat.mul_sub_distr_r. auto.
-      - eauto.
-      - cancel. apply LOG.intact_hashmap_subset. eauto.
-      Grab Existential Variables.
-      all : eauto; try split; eauto.
-  Qed.
-
-  Hint Extern 1 ({{_}} Bind (indshrink_aligned _ _ _ _ _ _ _) _) => apply indshrink_aligned_ok : prog.
-
-  Fixpoint indshrink_ragged_to_aligned indlvl lxp bxp iblocks nvalid ms :=
-    let N := (NIndirect ^ indlvl) in
-    let ragged_bn := selN iblocks (nvalid / N) $0 in
-    match indlvl with
-    | 0 => Ret ^(ms)
-    | S indlvl' =>
-    let N' := NIndirect ^ indlvl' in
-      If (addr_eq_dec (nvalid mod N) 0) {
-        Ret ^(ms)
-      } else {
-        If (addr_eq_dec indlvl' 0) {
-          ms <- BALLOC.free lxp bxp #ragged_bn ms;
-          Ret ^(ms)
-        } else {
-          let^ (ms, indbns) <- IndRec.read lxp #ragged_bn 1 ms;
-          let^ (ms) <- indshrink_ragged_to_aligned indlvl' lxp bxp indbns (nvalid mod N) ms;
-          let nvalid' := (nvalid mod N) / N' * N' in
-          let^ (ms) <- indshrink_aligned indlvl' lxp bxp indbns nvalid' nvalid' ms;
-          ms <- BALLOC.free lxp bxp #ragged_bn ms;
-          Ret ^(ms)
-        }
-      }
-    end.
-
-  Theorem indshrink_ragged_to_aligned_ok : forall indlvl lxp bxp iblocks l_part nvalid ms,
-    let N := NIndirect ^ indlvl in
-    {< F Fm m0 m freelist,
-    PRE:hm
-           LOG.rep lxp F (LOG.ActiveTxn m0 m) ms hm *
-           [[ indlvl > 0 ]] *
-           [[[ m ::: (Fm *
-                listmatch (fun index_ibn' l' => let '(index, ibn') := index_ibn' in
-                    indrep_n_tree (indlvl - 1) bxp (# ibn') l' (index_nvalid (indlvl - 1) nvalid index))
-                  (enumerate iblocks) l_part * BALLOC.rep bxp freelist) ]]] *
-           [[ length iblocks = NIndirect ]] * [[ nvalid <= NIndirect * N ]]
-    POST:hm' RET:^(ms)  exists m' freelist' nvalid',
-           [[ nvalid' = (nvalid / N * N)%nat]] *
-           LOG.rep lxp F (LOG.ActiveTxn m0 m') ms hm' *
-           [[[ m' ::: (Fm *
-                listmatch (fun index_ibn' l' => let '(index, ibn') := index_ibn' in
-                    indrep_n_tree (indlvl - 1) bxp (# ibn') l' (index_nvalid (indlvl - 1) nvalid' index))
-                  (enumerate iblocks) l_part * BALLOC.rep bxp freelist') ]]] *
-           [[ incl freelist freelist' ]]
-    CRASH:hm'  LOG.intact lxp F m0 hm'
-    >} indshrink_ragged_to_aligned indlvl lxp bxp iblocks nvalid ms.
-    Proof.
-      destruct indlvl.
-      simpl. hoare.
-      induction indlvl.
-      + simpl. rewrite mult_1_r.
-        step; [> step |]. rewrite mul_div by auto. cancel.
-        destruct (addr_eq_dec (nvalid mod NIndirect) 0); [> hoare |].
-        assert (nvalid / NIndirect < NIndirect).
-          match goal with [H : nvalid <= NIndirect * NIndirect |- _] =>
-            apply le_lt_eq_dec in H; destruct H
-          end; [> apply Nat.div_lt_upper_bound; auto; congruence | subst].
-          rewrite Nat.mod_mul in * by auto. omega.
-        assert (nvalid > 0) by (eapply lt_le_trans; [> apply neq_0_lt | apply Nat.mod_le]; eauto).
-        hoare.
-        - rewrite listmatch_extract with (i := nvalid / NIndirect) in *;
-            autorewrite with lists in *; destruct_lifts; try omega.
-          unfold index_nvalid in *. rewrite Nat.pow_1_r in *.
-          rewrite sub_round_eq_mod in * by auto.
-          rewrite nvalid_gt_0_indrep_helper in * by omega.
-          destruct_lifts. erewrite snd_pair in * by auto. eauto.
-        - rewrite listmatch_length_pimpl. cancel.
-          indrep_n_extract.
-          indrep_n_extract.
-          rewrite listmatch_indrep_n_tree_replace_nvalid with (indlvl := 0). cancel.
-          unfold index_nvalid; rewrite Nat.pow_1_r.
-          rewrite sub_round_eq_mod by auto.
-          rewrite indrep_n_helper_pts_piff by omega.
-          rewrite Nat.sub_diag, indrep_n_helper_0. cancel.
-          unfold IndRec.items_valid, IndSig.RALen in *. rewrite mult_1_l in *. intuition. eauto.
-          rewrite Nat.pow_1_r. auto.
-          rewrite Nat.pow_1_r. rewrite Nat.div_mul by auto. auto.
-      + (* simpl makes things messy if (S indlvl) carries through *)
-        remember (S indlvl) as I. assert (I + 0 = S indlvl) by omega. clear HeqI.
-        unfold indshrink_ragged_to_aligned. fold indshrink_ragged_to_aligned.
-        remember (S I) as II. assert (II + 0 = S I + 0) by omega. clear HeqII.
-        step; [> step |]. rewrite mul_div by mult_nonzero. auto.
-        step; [> step |].
-        rewrite listmatch_length_pimpl in *; autorewrite with lists in *; destruct_lifts.
-        match goal with [H : nvalid <= _ |- _] =>
-          apply le_lt_eq_dec in H; destruct H;
-          [>| subst nvalid; rewrite Nat.mod_mul in * by mult_nonzero; omega]
-        end.
-        match goal with [H : context [listmatch _ (enumerate ?l) _] |- context [selN ?l ?n] ] =>
-          rewrite listmatch_extract with (i := n) in H; autorewrite with lists in *;
-          replace II with (S (S (I - 1))) in H at 3 by omega; simpl in H; destruct_lift H
-        end; try (apply Nat.div_lt_upper_bound; mult_nonzero; rewrite mult_comm; congruence).
-        erewrite snd_pair in * by eauto.
-        step.
-        rewrite nvalid_gt_0_indrep_helper. cancel.
-        apply divup_gt_0; mult_nonzero. unfold index_nvalid.
-        repeat rewrite sub_S_1 by omega. rewrite sub_round_eq_mod by mult_nonzero. omega.
-        rewrite indrep_n_helper_length_piff, listmatch_length_pimpl with (a := enumerate _) in *.
-        destruct_lifts. autorewrite with lists in *.
-        rewrite firstn_oob by omega.
-        repeat safestep.
-        - unfold index_nvalid. repeat rewrite sub_S_1 by omega. rewrite sub_round_eq_mod by mult_nonzero.
-          cancel.
-        -replace II with (S I) by omega. auto.
-        - cancel.
-        - eapply le_trans; [> apply div_mul_le |]. replace II with (S I) by omega. auto.
-        - rewrite nvalid_gt_0_indrep_helper with (nvalid := divup _ _) in * by
-          (apply divup_gt_0; mult_nonzero; omega).
-          match goal with [H : context [?P] |- ?P] => destruct_lift H; auto end.
-        - rewrite Nat.sub_diag; simpl.
-          rewrite indrep_n_helper_pts_piff by (apply divup_gt_0; mult_nonzero; omega).
-          cancel.
-          assert (nvalid / NIndirect ^ II < NIndirect) by (apply Nat.div_lt_upper_bound; auto; rewrite mult_comm; auto).
-          indrep_n_extract.
-          rewrite listmatch_indrep_n_tree_replace_nvalid.
-          unfold index_nvalid. repeat rewrite sub_S_1 by omega.
-          rewrite Nat.sub_diag, indrep_n_tree_0. cancel.
-          apply listmatch_emp.
-          intros x; destruct x; intros. unfold index_nvalid. rewrite indrep_n_tree_0. cancel.
-          match goal with [H : ?l = _ |- _] => rewrite H end.
-          replace (II - 1) with (S (I - 1)) by omega.
-          eapply indrep_n_tree_length.
-          match goal with [H : context [listmatch _ _ ?l] |- context [listmatch _ _ ?l] ] =>
-            eapply pimpl_apply; [> | exact H]; cancel
-          end.
-          repeat match goal with
-          | [|- _ * _ =p=> _ * _] => apply pimpl_refl
-          | [|- (_ * _) * _ =p=> _ ] => rewrite sep_star_comm
-          | [|- _ * (_ * _) =p=> _ ] => repeat rewrite <- sep_star_assoc
-          end.
-          rewrite sub_S_1 by omega. rewrite Nat.div_mul; auto.
-          rewrite sub_S_1 by omega. auto.
-        - auto.
-        - apply incl_tl. eapply incl_tran; eauto.
-    Grab Existential Variables.
-    all : eauto; try split; eauto; solve [exact $0 | exact nil].
-  Qed.
-
-  Hint Extern 1 ({{_}} Bind (indshrink_ragged_to_aligned _ _ _ _ _ _) _) => apply indshrink_ragged_to_aligned_ok : prog.
-
-  Fixpoint indshrink_aligned_to_ragged indlvl lxp bxp iblocks nvalid nr ms :=
-    let N := (NIndirect ^ indlvl) in
-    let ragged_bn := (selN iblocks (nvalid / N - 1) $0) in
-    match indlvl with
-    | 0 => Ret ^(ms)
-    | S indlvl' =>
-      let N' := NIndirect ^ indlvl' in
-      If (addr_eq_dec indlvl' 0) {
-        Ret ^(ms)
-      } else {
-        If (addr_eq_dec nr 0) {
-          Ret ^(ms)
-        } else {
-          let^ (ms, indbns) <- IndRec.read lxp #ragged_bn 1 ms;
-          let^ (ms) <- indshrink_aligned indlvl' lxp bxp indbns N (nr / N' * N') ms;
-          let^ (ms) <- indshrink_aligned_to_ragged indlvl' lxp bxp indbns (N - (nr / N' * N')) (nr mod N') ms;
-          Ret ^(ms)
-        }
-      }
-    end.
-
-  Theorem indshrink_aligned_to_ragged_ok : forall indlvl lxp bxp iblocks l_part nvalid nr ms,
-    let N := NIndirect ^ indlvl in
-    {< F Fm m0 m freelist,
-    PRE:hm
-           LOG.rep lxp F (LOG.ActiveTxn m0 m) ms hm *
-           [[[ m ::: (Fm *
-                listmatch (fun index_ibn' l' => let '(index, ibn') := index_ibn' in
-                    indrep_n_tree (indlvl - 1) bxp (# ibn') l' (index_nvalid (indlvl - 1) nvalid index))
-                  (enumerate iblocks) l_part * BALLOC.rep bxp freelist) ]]] *
-           [[ indlvl > 0 ]] * [[ length iblocks = NIndirect ]] * [[ nvalid <= NIndirect * N ]] *
-           [[ Nat.divide N nvalid ]] * [[ nr < N ]] * [[ nr <= nvalid ]]
-    POST:hm' RET:^(ms)  exists m' freelist',
-           LOG.rep lxp F (LOG.ActiveTxn m0 m') ms hm' *
-           [[[ m' ::: (Fm *
-                listmatch (fun index_ibn' l' => let '(index, ibn') := index_ibn' in
-                    indrep_n_tree (indlvl - 1) bxp (# ibn') l' (index_nvalid (indlvl - 1) (nvalid - nr) index))
-                  (enumerate iblocks) l_part * BALLOC.rep bxp freelist') ]]] * [[ incl freelist freelist' ]]
-    CRASH:hm'  LOG.intact lxp F m0 hm'
-    >} indshrink_aligned_to_ragged indlvl lxp bxp iblocks nvalid nr ms.
-    Proof.
-      destruct indlvl. simpl. hoare. (* indlvl = 0 violates the precondition *)
-      unfold Nat.divide.
-      induction indlvl; intros.
-      + repeat rewrite Nat.pow_1_r. simpl. hoare.
-        apply listmatch_piff_replace.
-        intros. unfold index_nvalid. in_enumerate.
-        rewrite Nat.pow_1_r. rewrite sub_sub_comm.
-        rewrite <- Nat.mul_le_mono_pos_r in * by mult_nonzero.
-        rewrite <- Nat.mul_sub_distr_r.
-        match goal with [H : ?n < length _ |- context [?x - ?n] ] =>
-          destruct (le_lt_dec x n); [> replace (x - n) with 0 by omega |
-            assert ((x - n) * NIndirect >= NIndirect) by (apply mul_ge_r; omega)]
-        end; auto.
-        repeat rewrite nvalid_gt_0_indrep_helper by omega. auto.
-      + remember (S indlvl) as I. assert (I > 0) by omega. clear HeqI.
-        simpl.
-        step; [> hoare |].
-        rewrite <- Nat.mul_le_mono_pos_r in * by mult_nonzero.
-        repeat rewrite Nat.div_mul in * by mult_nonzero.
-        step; [> hoare |]. repeat rewrite Nat.sub_0_r. auto.
-        match goal with [H : nr <= ?n' * ?N |- _] =>
-          destruct (addr_eq_dec n' 0); [> solve [subst; simpl in *; step]|]
-        end.
-        match goal with [H : context [listmatch _ (enumerate ?l)]|- context [selN ?l ?n] ] =>
-          rewrite listmatch_extract with (i := n) in H; destruct_lift H;
-          autorewrite with lists in *; try omega
-        end.
-        match goal with [H : context [indrep_n_tree ?I ?bxp # (selN ?l ?n ?d)] |- _] =>
-          replace (indrep_n_tree I bxp #(selN l n d)) with (indrep_n_tree (S (I - 1)) bxp #(selN l n d))
-            in H by (f_equal; omega); simpl in H; destruct_lift H
-        end.
-        repeat rewrite Nat.sub_0_r in *.
-        step.
-        rewrite nvalid_gt_0_indrep_helper. erewrite snd_pair by eauto. cancel.
-        apply divup_gt_0; mult_nonzero.
-        unfold index_nvalid. simpl. rewrite <- Nat.mul_sub_distr_r.
-        mult_nonzero; omega.
-        rewrite indrep_n_helper_length_piff in *. destruct_lifts.
-        rewrite firstn_oob by omega.
-        step.
-        unfold index_nvalid. repeat rewrite sub_S_1 by omega.
-        rewrite <- Nat.mul_sub_distr_r. rewrite sub_sub_assoc by omega.
-        rewrite mult_1_l. cancel.
-        rewrite <- Nat.mul_le_mono_pos_r by mult_nonzero.
-        apply Nat.div_le_upper_bound; mult_nonzero. rewrite mult_comm; omega.
-        step.
-        rewrite <- Nat.mul_sub_distr_r by mult_nonzero.
-        match goal with [H : nr < ?n * ?N |- context [nr / ?N] ] =>
-          rewrite mult_comm in H; apply Nat.div_lt_upper_bound in H; mult_nonzero
-        end. apply mult_le_compat_r; mult_nonzero. omega.
-        rewrite <- Nat.mul_sub_distr_r by mult_nonzero. eauto.
-        apply Nat.mod_upper_bound; mult_nonzero.
-        eapply le_trans. apply mod_le_r.
-        rewrite <- Nat.mul_sub_distr_r. apply mul_ge_r.
-        apply Nat.lt_add_lt_sub_r; simpl.
-        apply Nat.div_lt_upper_bound; mult_nonzero.
-        rewrite mult_comm. auto.
-        hoare.
-        rewrite <- Nat.sub_add_distr.
-        rewrite mult_comm with (n := _ / _).
-        rewrite <- Nat.div_mod by mult_nonzero.
-        indrep_n_extract.
-        unfold index_nvalid.
-        replace (NIndirect * NIndirect ^ (I - 1)) with (NIndirect ^ (S (I -1))) by auto.
-        unfold index_nvalid. replace (S (I - 1)) with I by omega. simpl.
-        rewrite sub_sub_comm.
-        repeat rewrite <- Nat.mul_sub_distr_r.
-        rewrite sub_sub_assoc by omega. rewrite mult_1_l.
-        rewrite divup_mul by mult_nonzero.
-        rewrite listmatch_piff_replace. cancel.
-        replace (indrep_n_tree I) with (indrep_n_tree (S (I - 1))) by (f_equal; omega). simpl.
-        unfold index_nvalid. rewrite sub_S_1 by omega. simpl.
-        cancel; eauto.
-        rewrite nvalid_gt_0_indrep_helper by auto.
-        rewrite nvalid_gt_0_indrep_helper by (apply divup_gt_0; mult_nonzero; omega). cancel.
-        intros. in_enumerate.
-        rewrite sub_sub_comm. rewrite <- Nat.mul_sub_distr_r. intuition.
-        rewrite indrep_n_tree_nvalid_oob by (simpl; apply mul_ge_r; mult_nonzero; omega).
-        rewrite indrep_n_tree_nvalid_oob with (nvalid := _ - _). auto.
-        simpl.
-        match goal with [|- ?n * ?N - ?nr >= ?N] =>
-          apply Nat.le_add_le_sub_r; eapply le_trans with (m := 2 * N)
-        end; try omega. rewrite <- Nat.mul_le_mono_pos_r by mult_nonzero. omega.
-        rewrite sub_le_eq_0 by omega. auto.
-        eapply incl_tran; eauto.
-        Unshelve. all : eauto.
+      unfold indput_get_blocks. unfold indrep_n_helper. intros.
+      hoare. destruct_lifts. auto.
+      destruct addr_eq_dec; try omega. cancel.
+      apply firstn_oob.
+      unfold IndRec.rep, IndRec.items_valid, IndSig.RALen in *.
+      destruct addr_eq_dec; destruct_lifts.
+      rewrite repeat_length. omega.
+      omega.
     Qed.
 
-  Hint Extern 1 ({{_}} Bind (indshrink_aligned_to_ragged _ _ _ _ _ _ _) _) => apply indshrink_aligned_to_ragged_ok : prog.
+  Local Hint Extern 0 ({{_}} Bind (indput_get_blocks _ _ _ _) _) => apply indput_get_blocks_ok : prog.
 
-  Fixpoint indshrink indlvl lxp bxp ir nvalid nr ms :=
-    match indlvl with
-    | 0 => If (addr_eq_dec nvalid nr) {
-             ms <- BALLOC.free lxp bxp ir ms;
-             Ret ^(ms)
-           } else {
-             Ret ^(ms)
-           }
-    | S indlvl' =>
-      let N := (NIndirect ^ indlvl) in
-      let^ (ms, indbns) <- IndRec.read lxp ir 1 ms;
-      let last_block := divup nvalid N - 1 in
-      If (le_dec nr (nvalid mod N)) {
-        let^ (ms) <- indshrink indlvl' lxp bxp #(selN indbns last_block $0) (nvalid mod N) nr ms;
-        If (addr_eq_dec nvalid nr) {
-          ms <- BALLOC.free lxp bxp ir ms;
-          Ret ^(ms)
-        } else {
-          Ret ^(ms)
-        }
-      } else {
-        let^ (ms) <- indshrink_ragged_to_aligned (S indlvl') lxp bxp indbns nvalid ms;
-        (* the number of valid blocks is now aligned to a child boundary *)
-        let nvalid' := (nvalid / N * N) in
-        let nr' := (nr - (nvalid mod N)) in
-        let^ (ms) <- indshrink_aligned (S indlvl') lxp bxp indbns nvalid' (nr' / N * N) ms;
-        (* there is at most one more block that needs to be shrunk *)
-        let^ (ms) <- indshrink_aligned_to_ragged (S indlvl') lxp bxp indbns (roundup (nvalid - nr) N) (nr' mod N) ms;
-        If (addr_eq_dec nvalid nr) {
-          ms <- BALLOC.free lxp bxp ir ms;
-          Ret ^(ms)
-        } else {
-          Ret ^(ms)
-        }
-      }
-    end.
-
-  Theorem indshrink_ok : forall indlvl lxp bxp ir nvalid nr ms,
-    {< F Fm m0 m l freelist,
+  Theorem IndRec_write_no_rep_ok : forall lxp xp items ms,
+    {< F Fm m0 m old,
     PRE:hm
-           LOG.rep lxp F (LOG.ActiveTxn m0 m) ms hm *
-           [[[ m ::: (Fm * indrep_n_tree indlvl bxp ir l nvalid * BALLOC.rep bxp freelist) ]]] *
-           [[ nvalid <= length l ]] * [[0 < nr <= nvalid ]]
-    POST:hm' RET:^(ms)  exists m' freelist' nvalid',
-           [[ nvalid' = nvalid - nr ]] *
-           LOG.rep lxp F (LOG.ActiveTxn m0 m') ms hm' *
-           [[[ m' ::: (Fm * indrep_n_tree indlvl bxp ir l nvalid' * BALLOC.rep bxp freelist') ]]] *
-           [[ incl freelist freelist' ]]
-    CRASH:hm'  LOG.intact lxp F m0 hm'
-    >} indshrink indlvl lxp bxp ir nvalid nr ms.
+          LOG.rep lxp F (LOG.ActiveTxn m0 m) ms hm *
+          [[ IndRec.items_valid xp items ]] * [[ xp <> 0 ]] *
+          [[[ m ::: Fm * arrayN (@ptsto _ addr_eq_dec _) xp [old] ]]]
+    POST:hm' RET:ms' exists m',
+          LOG.rep lxp F (LOG.ActiveTxn m0 m') ms' hm' *
+          [[[ m' ::: Fm * IndRec.rep xp items ]]]
+    CRASH:hm' LOG.intact lxp F m0 hm'
+    >} IndRec.write lxp xp items ms.
   Proof.
-    induction indlvl.
-    + simpl. hoare.
-      - rewrite nvalid_gt_0_indrep_helper in * by omega. destruct_lifts; auto.
-      - rewrite indrep_n_helper_length_piff, indrep_n_helper_pts_piff by omega.
-        rewrite Nat.sub_diag, indrep_n_helper_0.
-        cancel.
-      - repeat rewrite nvalid_gt_0_indrep_helper by omega. cancel.
-    + unfold indshrink; fold indshrink.
-      remember (S indlvl) as I. rewrite <- plus_0_r with (n := I) in HeqI.
-      replace (indrep_n_tree I) with (indrep_n_tree (S (I - 1))) by (f_equal; omega).
-      step.
-      rewrite nvalid_gt_0_indrep_helper. cancel.
-      apply divup_gt_0; mult_nonzero; omega.
-      rewrite indrep_n_helper_length_piff in *; destruct_lifts.
-      rewrite firstn_oob by omega.
-      erewrite indrep_n_tree_length in * by (eapply pimpl_apply; [> | exact H]; cancel;
-        rewrite sep_star_comm; rewrite <- sep_star_assoc; apply pimpl_refl).
-      step.
-      - match goal with [|- context [nvalid mod ?N] ] =>
-          destruct (addr_eq_dec 0 (nvalid mod N)); [> substl (nvalid mod N) |]
-        end; [> solve [step] |].
-        rewrite divup_sub_1_eq by mult_nonzero.
-        replace (I - 1) with indlvl in * by omega. replace I with (S indlvl) in * by omega.
-        match goal with [H : nvalid <= NIndirect * ?N |- _] =>
-          apply le_lt_eq_dec in H; destruct H as [H | H];
-            [> | subst nvalid; rewrite Nat.mod_mul in * by mult_nonzero; omega];
-            assert (nvalid / N < NIndirect) by (apply Nat.div_lt_upper_bound; mult_nonzero;
-              rewrite mult_comm; congruence)
-        end.
-        rewrite listmatch_length_pimpl in *; autorewrite with lists in *. destruct_lifts.
-        repeat safestep.
-        --  indrep_n_extract.
-            unfold index_nvalid at 2.
-            rewrite sub_round_eq_mod by mult_nonzero. cancel.
-        --  eapply le_trans. apply mod_le_r.
-            apply Nat.eq_le_incl. symmetry.
-            apply Forall_selN; try omega.
-            eapply indrep_n_indlist_forall_length;
-            match goal with
-            [H : _ |- _] => solve [eapply pimpl_apply; [> | exact H]; cancel;
-              rewrite sep_star_comm, <- sep_star_assoc; eapply pimpl_refl]
-            end.
-        --  rewrite nvalid_gt_0_indrep_helper in * by (apply divup_gt_0; mult_nonzero).
-            destruct_lifts. auto.
-        --  match goal with [|- context [nr / ?N] ] =>
-              assert (nr < N) by (eapply le_lt_trans; [> eauto | apply Nat.mod_upper_bound]; mult_nonzero)
-            end.
-            rewrite Nat.div_small by auto.
-            rewrite divup_0. rewrite indrep_n_helper_0.
-            rewrite indrep_n_helper_length_piff, indrep_n_helper_pts_piff by (apply divup_gt_0; mult_nonzero).
-            cancel; eauto.
-            indrep_n_extract.
-            rewrite listmatch_indrep_n_tree_replace_nvalid. cancel.
-            unfold index_nvalid. simpl.
-            rewrite sub_le_eq_0 by (apply Nat.mod_le; mult_nonzero). cancel.
-            rewrite Nat.div_small; auto. rewrite Nat.div_0_l; mult_nonzero.
-            assert (NIndirect > 0) by auto. omega.
-        --  rewrite Nat.sub_diag. auto.
-        --  auto.
-        --  eauto.
-        --  indrep_n_extract.
-            repeat rewrite nvalid_gt_0_indrep_helper by (apply divup_gt_0; mult_nonzero; omega).
-            rewrite listmatch_indrep_n_tree_replace_nvalid. cancel.
-            unfold index_nvalid. rewrite sub_sub_comm, sub_round_eq_mod; mult_nonzero. cancel.
-            auto.
-            rewrite div_sub_small by mult_nonzero. auto.
-            omega.
-        --  auto.
-      - replace (NIndirect * NIndirect ^ (I - 1)) with (NIndirect ^ I) in *
-          by (destruct I; simpl; repeat f_equal; omega).
-        step. step.
-        apply mult_le_compat_r, Nat.div_le_mono. auto. omega.
-        apply mult_le_compat_r, Nat.div_le_upper_bound; mult_nonzero.
-        rewrite mult_comm; auto.
-        step.
-        rewrite <- roundup_sub_eq; auto; try omega. cancel.
-        eapply mod_reversed_ge; eauto; omega.
-        unfold roundup; apply mult_le_compat_r, divup_le. rewrite mult_comm; omega.
-        apply Nat.mod_bound_pos; (mult_nonzero || omega).
-        destruct (addr_eq_dec nvalid nr); subst.
-        rewrite sub_mod_eq_round, Nat.mod_mul by mult_nonzero.
-        rewrite Nat.sub_diag, roundup_0; auto.
-        eapply le_trans. eauto.
-        unfold roundup. apply mul_ge_r, divup_gt_0. omega. mult_nonzero.
-        rewrite sub_eq_roundup_sub by (mult_nonzero || omega).
-      repeat step.
-      --  rewrite nvalid_gt_0_indrep_helper in * by (apply divup_gt_0; mult_nonzero; omega).
-          destruct_lifts. auto.
-      --  rewrite Nat.sub_diag, divup_0. cancel.
-          rewrite indrep_n_helper_0, indrep_n_helper_length_piff.
-          rewrite indrep_n_helper_pts_piff by (apply divup_gt_0; mult_nonzero; omega).
-          cancel.
-      --  apply incl_tl. repeat (eapply incl_tran; eauto).
-      --  repeat rewrite nvalid_gt_0_indrep_helper by (apply divup_gt_0; mult_nonzero; omega). cancel.
-      --  repeat (eapply incl_tran; eauto).
-      Unshelve. all : eauto.
+    unfold IndRec.write, IndRec.rep, IndRec.items_valid.
+    hoare.
+    unfold IndSig.RAStart. instantiate (1 := [_]). cancel.
+    rewrite IndRec.Defs.ipack_one. auto.
+    unfold IndRec.Defs.item in *. simpl in *. omega.
+    rewrite vsupsyn_range_synced_list; auto.
+    rewrite IndRec.Defs.ipack_one. auto.
+    unfold IndRec.Defs.item in *. simpl in *. omega.
   Qed.
 
-  Fixpoint indgrow indlvl bxp lxp (ir : addr) nvalid bn ms :=
+  Local Hint Extern 0 ({{_}} Bind (IndRec.write _ _ _ _) _) => apply IndRec_write_no_rep_ok : prog.
+
+  Fixpoint indput indlvl bxp lxp root off bn ms :=
     let N := NIndirect ^ indlvl in
-    let^ (ms, ir) <- If (addr_eq_dec nvalid 0) {
-        let^ (ms, (r : option addr)) <- BALLOC.alloc lxp bxp ms;
-        Ret ^(ms, r)
+    let is_alloc := (addr_eq_dec root 0) in
+    let^ (ms, ir) <- If (is_alloc) {
+        BALLOC.alloc lxp bxp ms
       } else {
-        Ret ^(ms, Some ir)
+        Ret ^(ms, Some root)
       };
     match ir with
-    | None => Ret ^(ms, None)
+    | None => Ret ^(ms, 0)
     | Some ir =>
       match indlvl with
-      | 0 => ms <- IndRec.put lxp ir nvalid bn ms;
-        Ret ^(ms, Some ir)
+      | 0 => ms <- If (is_alloc) {
+                     IndRec.write lxp ir ((repeat $0 NIndirect) ⟦ off := bn ⟧) ms
+                   } else {
+                     IndRec.put lxp ir off bn ms
+                   };
+        Ret ^(ms, ir)
       | S indlvl' =>
-        let to_grow := nvalid / N in
-        let^ (ms, ir_to_grow) <- If (addr_eq_dec nvalid 0) {
+        let to_grow := off / N in
+        let^ (ms, indbns) <- indput_get_blocks lxp is_alloc ir ms;
+        let ir_to_grow := #(selN indbns to_grow $0) in
+        let^ (ms, v) <- indput indlvl' bxp lxp ir_to_grow (off mod N) bn ms;
+        If (addr_eq_dec v 0) {
           Ret ^(ms, 0)
         } else {
-          let^ (ms, indbns) <- IndRec.read lxp ir 1 ms;
-          Ret ^(ms, # (selN indbns to_grow $0))
-        };
-        let^ (ms, v) <- indgrow indlvl' bxp lxp ir_to_grow (nvalid mod N) bn ms;
-        match v with
-        | None => Ret ^(ms, None)
-        | Some v =>
-          If (addr_eq_dec v ir_to_grow) {
-            Ret ^(ms, Some ir)
-          } else {
-            ms <- IndRec.put lxp ir to_grow ($ v) ms;
-            Ret ^(ms, Some ir)
-          }
-        end
+          ms <- indput_upd_if_necessary lxp ir v indbns to_grow ms;
+          Ret ^(ms, ir)
+        }
       end
     end.
 
-  Theorem indgrow_ok : forall indlvl lxp bxp ir nvalid bn ms,
+  (* TODO move this *)
+  Theorem indrep_n_helper_pts_piff : forall bxp ir l,
+    ir <> 0 -> indrep_n_helper bxp ir l <=p=> [[ length l = NIndirect ]] *
+                [[ BALLOC.bn_valid bxp ir ]] * ir |-> (IndRec.Defs.block2val l, []).
+  Proof.
+    intros.
+    unfold indrep_n_helper, IndRec.rep. destruct addr_eq_dec; try omega.
+    unfold IndRec.items_valid, IndSig.xparams_ok, IndSig.RAStart, IndSig.RALen.
+    rewrite mult_1_l. unfold Rec.well_formed. simpl.
+    split; cancel;
+    rewrite IndRec.Defs.ipack_one by (unfold IndRec.Defs.item in *; auto).
+    all : cancel.
+  Qed.
+
+  (* TODO move to listutils *)
+  Lemma repeat_updN : forall T n (v : T) i, updN (repeat v n) i v = repeat v n.
+  Proof.
+    induction n; intros; simpl. auto.
+    destruct i. auto.
+    f_equal. auto.
+  Qed.
+
+  Theorem indput_ok : forall indlvl lxp bxp ir off bn ms,
     {< F Fm m0 m l freelist,
     PRE:hm
            LOG.rep lxp F (LOG.ActiveTxn m0 m) ms hm *
-           [[[ m ::: (Fm * indrep_n_tree indlvl bxp ir l nvalid * BALLOC.rep bxp freelist) ]]] *
-           [[ nvalid < length l ]]
-    POST:hm' RET:^(ms, r)
-           [[ r = None ]] * LOG.rep lxp F (LOG.ActiveTxn m0 m) ms hm' \/
-           exists m' freelist' ir' l' nvalid',
-           [[ r = Some ir' ]] * LOG.rep lxp F (LOG.ActiveTxn m0 m') ms hm' *
-           [[[ m' ::: (Fm * indrep_n_tree indlvl bxp ir' l' nvalid' * BALLOC.rep bxp freelist') ]]] *
-           [[ incl freelist' freelist ]] * [[ nvalid' = S nvalid ]] * [[ firstn nvalid l = firstn nvalid l' ]] *
-           [[ selN l' nvalid $0 = bn ]] * [[ nvalid = 0 \/ ir = ir' ]]
+           [[[ m ::: (Fm * indrep_n_tree indlvl bxp ir l * BALLOC.rep bxp freelist) ]]] *
+           [[ off < length l ]]
+    POST:hm' RET:^(ms, ir')
+           exists m', LOG.rep lxp F (LOG.ActiveTxn m0 m') ms hm' *
+           ([[ ir' = 0 ]] \/
+           exists freelist' l',
+           [[ ir = 0 \/ ir = ir' ]] *
+           [[[ m' ::: (Fm * indrep_n_tree indlvl bxp ir' l' * BALLOC.rep bxp freelist') ]]] *
+           [[ incl freelist' freelist ]] * [[ l' = updN l off bn ]])
     CRASH:hm'  LOG.intact lxp F m0 hm'
-    >} indgrow indlvl bxp lxp ir nvalid bn ms.
+    >} indput indlvl bxp lxp ir off bn ms.
     Proof.
       induction indlvl; intros; simpl.
-      + safestep.
-        - step.
-          unfold IndRec.put. rewrite Nat.div_0_l, Nat.mod_0_l by auto. unfold IndSig.RAStart.
-          hoare.
-          --  instantiate (1 := [_]). auto.
-          --  cancel.
-          --  instantiate (1 := [_]). cancel.
-          --  auto.
+      + step.
+        - hoare.
+          --  unfold IndRec.items_valid, IndSig.RAStart, IndSig.RALen, IndSig.xparams_ok.
+              rewrite mult_1_l. unfold Rec.well_formed. simpl. unfold BALLOC.bn_valid in *.
+              rewrite length_updN, repeat_length. intuition.
           --  unfold BALLOC.bn_valid in *. intuition.
-          --  or_r. cancel.
-              rewrite indrep_n_helper_0, indrep_n_helper_pts_piff by omega. cancel.
-              rewrite IndRec.Defs.block2val_updN_val2block_equiv by auto. cancel.
-              unfold IndRec.items_valid.
-              unfold IndSig.xparams_ok, IndSig.RAStart, Rec.well_formed. simpl.
-              unfold BALLOC.bn_valid in *. rewrite length_updN. intuition.
-              unfold IndRec.Defs.val2block, IndRec.Defs.blocktype.
-              rewrite (@Rec.array_of_word_length indrectype). auto.
+          --  or_r. cancel. unfold BALLOC.bn_valid in *; intuition.
+              rewrite indrep_n_helper_0. rewrite indrep_n_helper_valid by omega.
+              unfold BALLOC.bn_valid. cancel.
               apply incl_remove.
-              apply selN_updN_eq.
-              unfold IndRec.Defs.val2block, IndRec.Defs.blocktype.
-              rewrite (@Rec.array_of_word_length indrectype).
-              auto.
-      - monad_simpl. simpl.
-        hoare.
-        --  rewrite nvalid_gt_0_indrep_helper by omega. cancel.
-        --  or_r. safecancel.
-            eauto. rewrite nvalid_gt_0_indrep_helper. cancel.
-            rewrite nvalid_gt_0_indrep_helper in * by omega.
+        - hoare.
+        --  rewrite indrep_n_helper_valid by omega. cancel.
+        --  or_r. cancel.
+            rewrite indrep_n_helper_valid in * by omega. cancel.
             match goal with [H : context [?P] |- ?P] => destruct_lift H end. auto.
-            instantiate (1 := S _). omega.
-            auto.
-            symmetry. apply firstn_updN; auto.
-            apply selN_updN_eq.
-            omega.
-            auto.
-    Admitted.
+      + step.
+        - step. safestep.
+          rewrite repeat_selN, roundTrip_0. rewrite indrep_n_helper_0. rewrite indrep_n_tree_0. cancel.
+          eapply indrep_index_bound_helper; eauto.
+          match goal with [H : _ |- _] => 
+            eapply pimpl_apply; [> | exact H]; cancel; cancel_last
+          end.
+          rewrite repeat_length. apply Nat.mod_bound_pos; mult_nonzero; omega.
+          rewrite repeat_selN. rewrite roundTrip_0.
+          unfold indput_upd_if_necessary. rewrite repeat_selN, roundTrip_0.
+          hoare.
+          match goal with [H : BALLOC.bn_valid _ _ |- _] =>
+            let H' := fresh in (apply BALLOC.bn_valid_facts in H as H') end.
+          unfold IndRec.items_valid, IndSig.xparams_ok, IndSig.RAStart, IndSig.RALen, Rec.well_formed.
+          simpl. rewrite length_updN, repeat_length. intuition.
+          unfold BALLOC.bn_valid in *. intuition.
+          or_r.
+          norm. cancel. repeat split; auto.
+          pred_apply. norm; intuition.
+          instantiate (iblocks := updN _ _ _). cancel.
+          unfold BALLOC.bn_valid in *; intuition.
+          rewrite indrep_n_helper_valid by omega. cancel.
+          rewrite listmatch_updN_removeN.
+          indrep_n_extract. cancel.
+          rewrite repeat_selN, roundTrip_0. rewrite indrep_n_tree_0.
+          rewrite wordToNat_natToWord_idempotent'. cancel.
+          eapply BALLOC.bn_valid_goodSize; eauto.
+          (* TODO move this *)
+          Theorem indrep_n_tree_valid_piff : forall indlvl bxp ir l,
+            ir <> 0 -> indrep_n_tree indlvl bxp ir l <=p=> indrep_n_tree indlvl bxp ir l * [[ BALLOC.bn_valid bxp ir ]].
+          Proof.
+            destruct indlvl; intros; simpl.
+            repeat rewrite indrep_n_helper_valid by auto. split; cancel.
+            split; intros m' H'; destruct_lift H'; pred_apply; cancel.
+            rewrite indrep_n_helper_valid in * by auto. destruct_lifts. auto.
+          Qed.
+          rewrite indrep_n_tree_valid_piff in * by auto. destruct_lifts. auto.
+          all : try rewrite repeat_length; try solve [indrep_n_tree_bound |
+            eapply indrep_index_bound_helper; eauto;
+            match goal with [H : context [listmatch _ _ ?l] |- context [listmatch _ _ ?l] ] =>
+              eapply pimpl_apply; [> |exact H]; cancel end; rewrite indrep_n_helper_0; cancel].
+          unfold BALLOC.bn_valid. auto.
+          erewrite Nat.div_mod with (x := off) at 1.
+          rewrite plus_comm, mult_comm. rewrite updN_concat. f_equal.
+          match goal with [H : context [?l] |- context [selN ?l] ] =>
+            rewrite listmatch_extract with (b := l) in H
+          end. rewrite repeat_selN in *. rewrite roundTrip_0, indrep_n_tree_0 in *.
+          destruct_lifts.
+          match goal with [H : selN _ _ _ = _ |- _] => rewrite H end. reflexivity.
+          all : try rewrite repeat_length; try solve [indrep_n_tree_bound |
+            eapply indrep_index_bound_helper; eauto;
+            match goal with [H : context [listmatch _ _ ?l] |- context [listmatch _ _ ?l] ] =>
+              eapply pimpl_apply; [> |exact H]; cancel end; rewrite indrep_n_helper_0; cancel].
+          apply Nat.mod_bound_pos; mult_nonzero; omega.
+          eapply indrep_n_indlist_forall_length.
+          match goal with [H : context [listmatch _ _ ?l] |- context [listmatch _ _ ?l] ] =>
+            eapply pimpl_apply; [> |exact H]; cancel end. rewrite indrep_n_helper_0. cancel.
+          mult_nonzero.
+
+          (* TODO move this *)
+          Ltac incl_solve := match goal with
+          | [|- incl ?a ?a ] => apply incl_refl
+          | [|- incl (remove _ _ ?l) ?l ] => apply incl_remove
+          | [|- incl ?l (_ :: ?l)] => apply incl_tl; solve [incl_solve]
+          | [H : incl ?a ?b |- incl ?a ?c ] => eapply incl_tran; [> apply H|]; solve [incl_solve]
+          | [H : incl ?b ?c |- incl ?a ?c ] => eapply incl_tran; [> |apply H]; solve [incl_solve]
+          end.
+          Local Hint Extern 1 (incl ?a ?b) => incl_solve.
+          auto.
+          cancel.
+          or_l. cancel.
+        - monad_simpl. simpl. step.
+          rewrite indrep_n_helper_valid in * by auto. destruct_lifts. eauto.
+          cancel_last.
+          safestep.
+          indrep_n_extract; solve [cancel_last | indrep_n_tree_bound].
+          eapply lt_le_trans.
+          apply Nat.mod_bound_pos; mult_nonzero; omega.
+          apply Nat.eq_le_incl. symmetry. apply Forall_selN.
+          eapply indrep_n_indlist_forall_length.
+          match goal with [H : context [listmatch _ _ ?l] |- context [listmatch _ _ ?l] ] =>
+            eapply pimpl_apply; [> |exact H]; cancel end. cancel_last.
+          indrep_n_tree_bound.
+          step. step. step. step. step.
+          rewrite indrep_n_helper_valid in * by omega. destruct_lifts. auto.
+          step. or_r.
+          norm. cancel. repeat (split; try reflexivity). auto.
+          pred_apply. norm; intuition.
+          instantiate (iblocks := updN _ _ _). cancel.
+          rewrite listmatch_updN_removeN. cancel.
+          rewrite wordToNat_natToWord_idempotent'. cancel. apply pimpl_refl.
+          eapply BALLOC.bn_valid_goodSize; eauto.
+          rewrite indrep_n_tree_valid_piff in * by auto. destruct_lifts. auto.
+          indrep_n_tree_bound. indrep_n_tree_bound.
+          erewrite Nat.div_mod with (x := off) at 1.
+          rewrite plus_comm, mult_comm. rewrite updN_concat. reflexivity.
+          apply Nat.mod_bound_pos; mult_nonzero; omega.
+          eapply indrep_n_indlist_forall_length.
+          match goal with [H : context [listmatch _ _ ?l] |- context [listmatch _ _ ?l] ] =>
+            eapply pimpl_apply; [> |exact H]; cancel end. cancel_last.
+          mult_nonzero.
+          auto.
+          step. step.
+          rewrite indrep_n_helper_valid in * by omega. destruct_lifts. auto.
+          step.
+          or_r.
+          norm. cancel. repeat split. auto.
+          pred_apply. norm; intuition.
+          instantiate (iblocks := updN _ _ _). cancel.
+          rewrite listmatch_updN_removeN. cancel.
+          rewrite natToWord_wordToNat. cancel. apply pimpl_refl.
+          indrep_n_tree_bound.
+          indrep_n_tree_bound.
+          erewrite Nat.div_mod with (x := off) at 1.
+          rewrite plus_comm, mult_comm. rewrite updN_concat. reflexivity.
+          apply Nat.mod_bound_pos; mult_nonzero; omega.
+          eapply indrep_n_indlist_forall_length.
+          match goal with [H : context [listmatch _ _ ?l] |- context [listmatch _ _ ?l] ] =>
+            eapply pimpl_apply; [> |exact H]; cancel end. cancel_last.
+          mult_nonzero.
+          auto.
+          cancel.
+    Grab Existential Variables. all : auto; solve [exact nil | exact $0].
+  Qed.
 
   (************* program *)
 
